edits restruct

src/tls/TLSConstants.fst
@@ -155,99 +155,9 @@ let max_TLSCiphertext_fragment_length_13 = max_TLSPlaintext_fragment_length + 25
 (** Signature algorithms *)
 type sigAlg = CoreCrypto.sig_alg
 
-(* This is the old version of the inverse predicate. According to CF,
-   verification was harder with this style, so we moved to the new style with
-   pinverse_t + lemmas. The type abbrevations lemma_inverse_* minimize the
-   syntactic overhead.
-
-  logic type pinverse (#a:Type) (#b:Type) (r:b -> b -> Type) (=f:a -> Tot b) =
-    y:b -> Tot (xopt:result a{(forall (x:a). r (f x) y <==> (xopt = Correct x))})
-*)
-
-type pinverse_t (#a:Type) (#b:Type) ($f:(a -> Tot b)) = b -> Tot (result a)
-
-unfold type lemma_inverse_g_f (#a:Type) (#b:Type) ($f:a -> Tot b) ($g:b -> Tot (result a)) (x:a) =
-  g (f x) == Correct x
-
-unfold type lemma_pinverse_f_g (#a:Type) (#b:Type) (r:b -> b -> Type) ($f:a -> Tot b) ($g:b -> Tot (result a)) (y:b) =
-  is_Correct (g y) ==> r (f (Correct._0 (g y))) y
-
-
-(** Serializing function for signature algorithms *)
-val sigAlgBytes: sigAlg -> Tot (lbytes 1)
-let sigAlgBytes sa =
-  match sa with
-  | CoreCrypto.RSASIG -> abyte 1z
-  | CoreCrypto.DSA    -> abyte 2z
-  | CoreCrypto.ECDSA  -> abyte 3z
-  | CoreCrypto.RSAPSS -> abyte 0z // TODO fix me!
-
-(** Parsing function associated to sigAlgBytes *)
-val parseSigAlg: pinverse_t sigAlgBytes
-let parseSigAlg b =
-  match cbyte b with
-  | 1z -> Correct CoreCrypto.RSASIG
-  | 2z -> Correct CoreCrypto.DSA
-  | 3z -> Correct CoreCrypto.ECDSA
-  | 0z -> Correct CoreCrypto.RSAPSS
-  | _ -> Error (AD_decode_error, perror __SOURCE_FILE__ __LINE__ "")
-
-val inverse_sigAlg: x:_ -> Lemma
-  (requires (True))
-  (ensures lemma_inverse_g_f sigAlgBytes parseSigAlg x)
-  [SMTPat (parseSigAlg (sigAlgBytes x))]
-let inverse_sigAlg x = ()
-
-val pinverse_sigAlg: x:_ -> Lemma
-  (requires (True))
-  (ensures (lemma_pinverse_f_g Seq.equal sigAlgBytes parseSigAlg x))
-  [SMTPat (sigAlgBytes (Correct._0 (parseSigAlg x)))]
-let pinverse_sigAlg x = ()
-
 
 (** Hash algorithm minimum requirements *)
 type hashAlg' = h:hashAlg{h <> NULL /\ h <> MD5SHA1 }
-
-
-#set-options "--max_fuel 0 --initial_fuel 0 --max_ifuel 2 --initial_ifuel 2"
-
-(** Serializing of the Hash algorithm *)
-val hashAlgBytes: hashAlg' -> Tot (lbytes 1)
-let hashAlgBytes ha =
-  match ha with
-  | Hash MD5     -> abyte 1z
-  | Hash SHA1    -> abyte 2z
-  | Hash SHA224  -> abyte 3z
-  | Hash SHA256  -> abyte 4z
-  | Hash SHA384  -> abyte 5z
-  | Hash SHA512  -> abyte 6z
-  | NULL -> abyte 7z // FIXME!!
-
-(** Parsing of the Hash algorithm *)
-val parseHashAlg: pinverse_t hashAlgBytes
-let parseHashAlg b =
-  match cbyte b with
-  | 1z -> Correct (Hash MD5)
-  | 2z -> Correct (Hash SHA1)
-  | 3z -> Correct (Hash SHA224)
-  | 4z -> Correct (Hash SHA256)
-  | 5z -> Correct (Hash SHA384)
-  | 6z -> Correct (Hash SHA512)
-  | 7z -> admit();  //TODO: FIXME!!!!
-         Correct (NULL)
-  | _ -> Error (AD_decode_error, perror __SOURCE_FILE__ __LINE__ "")
-
-val inverse_hashAlg: x:_ -> Lemma
-  (requires (True))
-  (ensures lemma_inverse_g_f hashAlgBytes parseHashAlg x)
-  [SMTPat (parseHashAlg (hashAlgBytes x))]
-let inverse_hashAlg x = ()
-
-val pinverse_hashAlg: x:_ -> Lemma
-  (requires (True))
-  (ensures (lemma_pinverse_f_g Seq.equal hashAlgBytes parseHashAlg x))
-  [SMTPat (hashAlgBytes (Correct._0 (parseHashAlg x)))]
-let pinverse_hashAlg x = ()
 
 (** Encryption key sizes *)
 let encKeySize = function
@@ -293,22 +203,6 @@ let macSize = function
 type scsv_suite =
   | TLS_EMPTY_RENEGOTIATION_INFO_SCSV
 
-(* let known_cs_list = [( 0x00z, 0x00z ); *)
-(* ( 0x00z, 0x01z );( 0x00z, 0x02z ); ( 0x00z, 0x3Bz ); ( 0x00z, 0x04z ); ( 0x00z, 0x05z ); *)
-(* ( 0x00z, 0x0Az ); ( 0x00z, 0x2Fz ); ( 0x00z, 0x35z ); ( 0x00z, 0x3Cz );( 0x00z, 0x3Dz ); *)
-(*  ( 0x00z, 0x0Dz ); ( 0x00z, 0x10z ); ( 0x00z, 0x13z ); ( 0x00z, 0x16z ); *)
-(*  ( 0x00z, 0x30z ); ( 0x00z, 0x31z ); ( 0x00z, 0x32z ); ( 0x00z, 0x33z ); *)
-(*  ( 0x00z, 0x36z ); ( 0x00z, 0x37z ); ( 0x00z, 0x38z ); ( 0x00z, 0x39z ); *)
-(*  ( 0x00z, 0x3Ez ); ( 0x00z, 0x3Fz ); ( 0x00z, 0x40z ); ( 0x00z, 0x67z ); *)
-(*  ( 0x00z, 0x68z ); ( 0x00z, 0x69z ); ( 0x00z, 0x6Az ); ( 0x00z, 0x6Bz ); *)
-(*  ( 0xc0z, 0x11z ); ( 0xc0z, 0x12z ); ( 0xc0z, 0x13z ); ( 0xc0z, 0x14z ); ( 0xc0z, 0x27z ); ( 0xc0z, 0x28z ); *)
-(*  ( 0xc0z, 0x2fz ); ( 0xc0z, 0x30z ); *)
-(*  ( 0x00z, 0x18z ); ( 0x00z, 0x1Bz ); ( 0x00z, 0x34z ); ( 0x00z, 0x3Az ); ( 0x00z, 0x6Cz ); ( 0x00z, 0x6Dz ); *)
-(* ( 0x00z, 0x9Cz );( 0x00z, 0x9Dz ); *)
-(* ( 0x00z, 0x9Ez );( 0x00z, 0x9Fz );( 0x00z, 0xA0z );( 0x00z, 0xA1z ); *)
-(* ( 0x00z, 0xA2z );( 0x00z, 0xA3z );( 0x00z, 0xA4z );( 0x00z, 0xA5z ); *)
-(* ( 0x00z, 0xA6z ); ( 0x00z, 0xA7z ); ( 0x00z, 0xFFz )] *)
-
 (** Ciphersuite definition *)
 type cipherSuite =
   | NullCipherSuite: cipherSuite
@@ -324,84 +218,6 @@ type compression =
   | NullCompression
   | UnknownCompression of (b:byte{b <> 0z})
 
-(** Serializing function for compression algorithms *)
-val compressionBytes: compression -> Tot (lbytes 1)
-let compressionBytes comp =
-  match comp with
-  | NullCompression      -> abyte 0z
-  | UnknownCompression b -> abyte b
-
-// Not pinverse_t compressionBytes, because it never fails
-
-(** Parsing function for compression algorithm *)
-val parseCompression: b:lbytes 1
-  -> Tot (cm:compression{Seq.equal (compressionBytes cm) b})
-let parseCompression b =
-  match cbyte b with
-  | 0z -> NullCompression
-  | b  -> UnknownCompression b
-
-// We ignore compression methods we don't understand. This is a departure
-// from usual parsing, where we fail on unknown values, but that's how TLS
-// handles compression method lists.
-
-(** Parsing function for compression algorithm lists *)
-val parseCompressions: b:bytes -> Tot (list compression) (decreases (length b))
-let rec parseCompressions b =
-  if length b > 0
-  then
-    let cmB,b = split b 1 in
-    let cm = parseCompression cmB in
-    cm::(parseCompressions b)
-  else []
-
-
-#set-options "--max_fuel 1 --initial_fuel 1 --max_ifuel 1 --initial_ifuel 1"
-
-(** Serializing function for lists of compression algorithms *)
-val compressionMethodsBytes: cms:list compression
-  -> Tot (lbytes (List.Tot.length cms))
-let rec compressionMethodsBytes cms =
-  match cms with
-  | c::cs -> compressionBytes c @| compressionMethodsBytes cs
-  | []   -> empty_bytes
-
-
-#set-options "--max_fuel 0 --initial_fuel 0 --max_ifuel 1 --initial_ifuel 1"
-
-(** Serializing function for the protocol version *)
-val versionBytes: protocolVersion -> Tot (lbytes 2)
-let versionBytes pv =
-  match pv with
-  | SSL_3p0 -> abyte2 ( 3z, 0z)
-  | TLS_1p0 -> abyte2 ( 3z, 1z)
-  | TLS_1p1 -> abyte2 ( 3z, 2z )
-  | TLS_1p2 -> abyte2 ( 3z, 3z )
-  | TLS_1p3 -> abyte2 ( 3z, 4z )
-
-(** Parsing function for the protocol version *)
-val parseVersion: pinverse_t versionBytes
-let parseVersion v =
-  match cbyte2 v with
-  | ( 3z, 0z ) -> Correct SSL_3p0
-  | ( 3z, 1z ) -> Correct TLS_1p0
-  | ( 3z, 2z ) -> Correct TLS_1p1
-  | ( 3z, 3z ) -> Correct TLS_1p2
-  | ( 3z, 4z ) -> Correct TLS_1p3
-  | _ -> Error(AD_decode_error, perror __SOURCE_FILE__ __LINE__ "Parsed an unknown version")
-
-val inverse_version: x:_ -> Lemma
-  (requires (True))
-  (ensures lemma_inverse_g_f versionBytes parseVersion x)
-  [SMTPat (parseVersion (versionBytes x))]
-let inverse_version x = ()
-
-val pinverse_version: x:_ -> Lemma
-  (requires (True))
-  (ensures (lemma_pinverse_f_g Seq.equal versionBytes parseVersion x))
-  [SMTPat (versionBytes (Correct._0 (parseVersion x)))]
-let pinverse_version x = ()
-
 (** Determine the oldest protocol versions for TLS *)
 let minPV (a:protocolVersion) (b:protocolVersion) =
   match a,b with
@@ -412,298 +228,6 @@ let minPV (a:protocolVersion) (b:protocolVersion) =
   | TLS_1p3, _  | _, TLS_1p3 -> TLS_1p3
 
 let geqPV a b = (b = minPV a b)
-
-(* JK: injectivity proof requires extra specification for the UnknownCipherSuite objects as they
-   have to be distinct from the 'correct' ones *)
-val cipherSuiteBytesOpt: cipherSuite -> Tot (option (lbytes 2))
-let cipherSuiteBytesOpt cs =
-  let abyte2 b: option (lbytes 2) = Some (abyte2 b) in
-    match cs with
-    | UnknownCipherSuite b1 b2 -> abyte2 (b1,b2)
-    | NullCipherSuite                                              -> abyte2 ( 0x00z, 0x00z )
-
-    | CipherSuite Kex_RSA None (MACOnly MD5)                       -> abyte2 ( 0x00z, 0x01z )
-    | CipherSuite Kex_RSA None (MACOnly SHA1)                      -> abyte2 ( 0x00z, 0x02z )
-    | CipherSuite Kex_RSA None (MACOnly SHA256)                    -> abyte2 ( 0x00z, 0x3Bz )
-    | CipherSuite Kex_RSA None(MtE (Stream RC4_128) MD5)           -> abyte2 ( 0x00z, 0x04z )
-    | CipherSuite Kex_RSA None(MtE (Stream RC4_128) SHA1)          -> abyte2 ( 0x00z, 0x05z )
-
-    | CipherSuite Kex_RSA None(MtE (Block TDES_EDE_CBC) SHA1)      -> abyte2 ( 0x00z, 0x0Az )
-    | CipherSuite Kex_RSA None(MtE (Block AES_128_CBC) SHA1)       -> abyte2 ( 0x00z, 0x2Fz )
-    | CipherSuite Kex_RSA None(MtE (Block AES_256_CBC) SHA1)       -> abyte2 ( 0x00z, 0x35z )
-    | CipherSuite Kex_RSA None(MtE (Block AES_128_CBC) SHA256)     -> abyte2 ( 0x00z, 0x3Cz )
-    | CipherSuite Kex_RSA None(MtE (Block AES_256_CBC) SHA256)     -> abyte2 ( 0x00z, 0x3Dz )
-
-    (**************************************************************************)
-    | CipherSuite Kex_DH (Some DSA)     (MtE (Block TDES_EDE_CBC) SHA1)   -> abyte2 ( 0x00z, 0x0Dz )
-    | CipherSuite Kex_DH (Some RSASIG)  (MtE (Block TDES_EDE_CBC) SHA1)   -> abyte2 ( 0x00z, 0x10z )
-    | CipherSuite Kex_DHE (Some DSA)    (MtE (Block TDES_EDE_CBC) SHA1)   -> abyte2 ( 0x00z, 0x13z )
-    | CipherSuite Kex_DHE (Some RSASIG) (MtE (Block TDES_EDE_CBC) SHA1)   -> abyte2 ( 0x00z, 0x16z )
-
-    | CipherSuite Kex_DH (Some DSA)     (MtE (Block AES_128_CBC) SHA1)    -> abyte2 ( 0x00z, 0x30z )
-    | CipherSuite Kex_DH (Some RSASIG)  (MtE (Block AES_128_CBC) SHA1)    -> abyte2 ( 0x00z, 0x31z )
-    | CipherSuite Kex_DHE (Some DSA)    (MtE (Block AES_128_CBC) SHA1)    -> abyte2 ( 0x00z, 0x32z )
-    | CipherSuite Kex_DHE (Some RSASIG) (MtE (Block AES_128_CBC) SHA1)    -> abyte2 ( 0x00z, 0x33z )
-
-    | CipherSuite Kex_DH (Some DSA)     (MtE (Block AES_256_CBC) SHA1)    -> abyte2 ( 0x00z, 0x36z )
-    | CipherSuite Kex_DH (Some RSASIG)  (MtE (Block AES_256_CBC) SHA1)    -> abyte2 ( 0x00z, 0x37z )
-    | CipherSuite Kex_DHE (Some DSA)    (MtE (Block AES_256_CBC) SHA1)    -> abyte2 ( 0x00z, 0x38z )
-    | CipherSuite Kex_DHE (Some RSASIG) (MtE (Block AES_256_CBC) SHA1)    -> abyte2 ( 0x00z, 0x39z )
-
-    | CipherSuite Kex_DH (Some DSA)     (MtE (Block AES_128_CBC) SHA256)  -> abyte2 ( 0x00z, 0x3Ez )
-    | CipherSuite Kex_DH (Some RSASIG)  (MtE (Block AES_128_CBC) SHA256)  -> abyte2 ( 0x00z, 0x3Fz )
-    | CipherSuite Kex_DHE (Some DSA)    (MtE (Block AES_128_CBC) SHA256)  -> abyte2 ( 0x00z, 0x40z )
-    | CipherSuite Kex_DHE (Some RSASIG) (MtE (Block AES_128_CBC) SHA256)  -> abyte2 ( 0x00z, 0x67z )
-
-    | CipherSuite Kex_DH (Some DSA)     (MtE (Block AES_256_CBC) SHA256)  -> abyte2 ( 0x00z, 0x68z )
-    | CipherSuite Kex_DH (Some RSASIG)  (MtE (Block AES_256_CBC) SHA256)  -> abyte2 ( 0x00z, 0x69z )
-    | CipherSuite Kex_DHE (Some DSA)    (MtE (Block AES_256_CBC) SHA256)  -> abyte2 ( 0x00z, 0x6Az )
-    | CipherSuite Kex_DHE (Some RSASIG) (MtE (Block AES_256_CBC) SHA256)  -> abyte2 ( 0x00z, 0x6Bz )
-
-    (**************************************************************************)
-    | CipherSuite Kex_ECDHE (Some RSASIG) (MtE (Stream RC4_128) SHA1)       -> abyte2 ( 0xc0z, 0x11z )
-    | CipherSuite Kex_ECDHE (Some RSASIG) (MtE (Block TDES_EDE_CBC) SHA1)   -> abyte2 ( 0xc0z, 0x12z )
-    | CipherSuite Kex_ECDHE (Some RSASIG) (MtE (Block AES_128_CBC) SHA1)    -> abyte2 ( 0xc0z, 0x13z )
-    | CipherSuite Kex_ECDHE (Some RSASIG) (MtE (Block AES_256_CBC) SHA1)    -> abyte2 ( 0xc0z, 0x14z )
-    | CipherSuite Kex_ECDHE (Some RSASIG) (MtE (Block AES_128_CBC) SHA256)  -> abyte2 ( 0xc0z, 0x27z )
-    | CipherSuite Kex_ECDHE (Some RSASIG) (MtE (Block AES_256_CBC) SHA384)  -> abyte2 ( 0xc0z, 0x28z )
-
-    | CipherSuite Kex_ECDHE (Some RSASIG) (AEAD AES_128_GCM SHA256) -> abyte2 ( 0xc0z, 0x2fz )
-    | CipherSuite Kex_ECDHE (Some ECDSA)  (AEAD AES_128_GCM SHA256) -> abyte2 ( 0xc0z, 0x2bz )
-    | CipherSuite Kex_ECDHE (Some RSASIG) (AEAD AES_256_GCM SHA384) -> abyte2 ( 0xc0z, 0x30z )
-    | CipherSuite Kex_ECDHE (Some ECDSA) (AEAD AES_256_GCM SHA384) -> abyte2 ( 0xc0z, 0x2cz )
-
-    (**************************************************************************)
-    | CipherSuite Kex_PSK_DHE None (AEAD AES_128_GCM SHA256) -> abyte2 ( 0x00z, 0xaaz )
-    | CipherSuite Kex_PSK_DHE None (AEAD AES_256_GCM SHA384) -> abyte2 ( 0x00z, 0xabz )
-    | CipherSuite Kex_PSK_ECDHE None (AEAD AES_128_GCM SHA256) -> abyte2 ( 0xd0z, 0x01z )
-    | CipherSuite Kex_PSK_ECDHE None (AEAD AES_256_GCM SHA384) -> abyte2 ( 0xd0z, 0x02z )
-
-    (**************************************************************************)
-    | CipherSuite Kex_DHE None   (MtE (Stream RC4_128) MD5)         -> abyte2 ( 0x00z, 0x18z )
-    | CipherSuite Kex_DHE None   (MtE (Block TDES_EDE_CBC) SHA1)    -> abyte2 ( 0x00z, 0x1Bz )
-    | CipherSuite Kex_DHE None   (MtE (Block AES_128_CBC) SHA1)     -> abyte2 ( 0x00z, 0x34z )
-    | CipherSuite Kex_DHE None   (MtE (Block AES_256_CBC) SHA1)     -> abyte2 ( 0x00z, 0x3Az )
-    | CipherSuite Kex_DHE None   (MtE (Block AES_128_CBC) SHA256)   -> abyte2 ( 0x00z, 0x6Cz )
-    | CipherSuite Kex_DHE None   (MtE (Block AES_256_CBC) SHA256)   -> abyte2 ( 0x00z, 0x6Dz )
-
-    (**************************************************************************)
-    | CipherSuite Kex_RSA None     (AEAD AES_128_GCM SHA256) -> abyte2( 0x00z, 0x9Cz )
-    | CipherSuite Kex_RSA None     (AEAD AES_256_GCM SHA384) -> abyte2( 0x00z, 0x9Dz )
-
-    | CipherSuite Kex_DHE (Some RSASIG) (AEAD AES_128_GCM SHA256) -> abyte2( 0x00z, 0x9Ez )
-    | CipherSuite Kex_DHE (Some RSASIG) (AEAD AES_256_GCM SHA384) -> abyte2( 0x00z, 0x9Fz )
-    | CipherSuite Kex_DH (Some RSASIG)  (AEAD AES_128_GCM SHA256) -> abyte2( 0x00z, 0xA0z )
-    | CipherSuite Kex_DH (Some RSASIG)  (AEAD AES_256_GCM SHA384) -> abyte2( 0x00z, 0xA1z )
-
-    | CipherSuite Kex_DHE (Some DSA) (AEAD AES_128_GCM SHA256) -> abyte2( 0x00z, 0xA2z )
-    | CipherSuite Kex_DHE (Some DSA) (AEAD AES_256_GCM SHA384) -> abyte2( 0x00z, 0xA3z )
-    | CipherSuite Kex_DH (Some DSA)  (AEAD AES_128_GCM SHA256) -> abyte2( 0x00z, 0xA4z )
-    | CipherSuite Kex_DH (Some DSA)  (AEAD AES_256_GCM SHA384) -> abyte2( 0x00z, 0xA5z )
-
-    | CipherSuite Kex_DHE None (AEAD AES_128_GCM SHA256) -> abyte2( 0x00z, 0xA6z )
-    | CipherSuite Kex_DHE None (AEAD AES_256_GCM SHA384) -> abyte2( 0x00z, 0xA7z )
-
-    | SCSV (TLS_EMPTY_RENEGOTIATION_INFO_SCSV)         -> abyte2 ( 0x00z, 0xFFz )
-    | _ -> None
-
-
-(** Determine if a ciphersuite is valid *)
-let validCipherSuite (c:cipherSuite) = is_Some (cipherSuiteBytesOpt c)
-let valid_cipher_suite = c:cipherSuite{validCipherSuite c}
-
-(** List of valid ciphersuite *)
-let valid_cipher_suites = list valid_cipher_suite
-
-(** Serializing function for a valid ciphersuite *)
-val cipherSuiteBytes: valid_cipher_suite -> Tot (lbytes 2)
-let cipherSuiteBytes c = Some.v (cipherSuiteBytesOpt c)
-
-#reset-options "--z3rlimit 60"
-
-(** Auxillary parsing function for ciphersuites *)
-val parseCipherSuiteAux : lbytes 2 -> Tot (result (c:cipherSuite{validCipherSuite c}))
-let parseCipherSuiteAux b =
-  match cbyte2 b with
-  | ( 0x00z, 0x00z ) -> Correct(NullCipherSuite)
-
-  | ( 0x00z, 0x01z ) -> Correct(CipherSuite Kex_RSA None (MACOnly MD5))
-  | ( 0x00z, 0x02z ) -> Correct(CipherSuite Kex_RSA None (MACOnly SHA1))
-  | ( 0x00z, 0x3Bz ) -> Correct(CipherSuite Kex_RSA None (MACOnly SHA256))
-  | ( 0x00z, 0x04z ) -> Correct(CipherSuite Kex_RSA None (MtE (Stream RC4_128) MD5))
-  | ( 0x00z, 0x05z ) -> Correct(CipherSuite Kex_RSA None (MtE (Stream RC4_128) SHA1))
-
-  | ( 0x00z, 0x0Az ) -> Correct(CipherSuite Kex_RSA None (MtE (Block TDES_EDE_CBC) SHA1))
-  | ( 0x00z, 0x2Fz ) -> Correct(CipherSuite Kex_RSA None (MtE (Block AES_128_CBC) SHA1))
-  | ( 0x00z, 0x35z ) -> Correct(CipherSuite Kex_RSA None (MtE (Block AES_256_CBC) SHA1))
-  | ( 0x00z, 0x3Cz ) -> Correct(CipherSuite Kex_RSA None (MtE (Block AES_128_CBC) SHA256))
-  | ( 0x00z, 0x3Dz ) -> Correct(CipherSuite Kex_RSA None (MtE (Block AES_256_CBC) SHA256))
-
-  (**************************************************************************)
-  | ( 0x00z, 0x0Dz ) -> Correct(CipherSuite Kex_DH (Some DSA) (MtE (Block TDES_EDE_CBC) SHA1))
-  | ( 0x00z, 0x10z ) -> Correct(CipherSuite Kex_DH (Some RSASIG) (MtE (Block TDES_EDE_CBC) SHA1))
-  | ( 0x00z, 0x13z ) -> Correct(CipherSuite Kex_DHE (Some DSA) (MtE (Block TDES_EDE_CBC) SHA1))
-  | ( 0x00z, 0x16z ) -> Correct(CipherSuite Kex_DHE (Some RSASIG) (MtE (Block TDES_EDE_CBC) SHA1))
-
-  | ( 0x00z, 0x30z ) -> Correct(CipherSuite Kex_DH (Some DSA) (MtE (Block AES_128_CBC) SHA1))
-  | ( 0x00z, 0x31z ) -> Correct(CipherSuite Kex_DH (Some RSASIG) (MtE (Block AES_128_CBC) SHA1))
-  | ( 0x00z, 0x32z ) -> Correct(CipherSuite Kex_DHE (Some DSA) (MtE (Block AES_128_CBC) SHA1))
-  | ( 0x00z, 0x33z ) -> Correct(CipherSuite Kex_DHE (Some RSASIG) (MtE (Block AES_128_CBC) SHA1))
-
-  | ( 0x00z, 0x36z ) -> Correct(CipherSuite Kex_DH (Some DSA) (MtE (Block AES_256_CBC) SHA1))
-  | ( 0x00z, 0x37z ) -> Correct(CipherSuite Kex_DH (Some RSASIG) (MtE (Block AES_256_CBC) SHA1))
-  | ( 0x00z, 0x38z ) -> Correct(CipherSuite Kex_DHE (Some DSA) (MtE (Block AES_256_CBC) SHA1))
-  | ( 0x00z, 0x39z ) -> Correct(CipherSuite Kex_DHE (Some RSASIG) (MtE (Block AES_256_CBC) SHA1))
-
-  | ( 0x00z, 0x3Ez ) -> Correct(CipherSuite Kex_DH (Some DSA) (MtE (Block AES_128_CBC) SHA256))
-  | ( 0x00z, 0x3Fz ) -> Correct(CipherSuite Kex_DH (Some RSASIG) (MtE (Block AES_128_CBC) SHA256))
-  | ( 0x00z, 0x40z ) -> Correct(CipherSuite Kex_DHE (Some DSA) (MtE (Block AES_128_CBC) SHA256))
-  | ( 0x00z, 0x67z ) -> Correct(CipherSuite Kex_DHE (Some RSASIG) (MtE (Block AES_128_CBC) SHA256))
-
-  | ( 0x00z, 0x68z ) -> Correct(CipherSuite Kex_DH (Some DSA) (MtE (Block AES_256_CBC) SHA256))
-  | ( 0x00z, 0x69z ) -> Correct(CipherSuite Kex_DH (Some RSASIG) (MtE (Block AES_256_CBC) SHA256))
-  | ( 0x00z, 0x6Az ) -> Correct(CipherSuite Kex_DHE (Some DSA) (MtE (Block AES_256_CBC) SHA256))
-  | ( 0x00z, 0x6Bz ) -> Correct(CipherSuite Kex_DHE (Some RSASIG) (MtE (Block AES_256_CBC) SHA256))
-
-  (**************************************************************************)
-  | ( 0xc0z, 0x11z ) -> Correct(CipherSuite Kex_ECDHE (Some RSASIG) (MtE (Stream RC4_128) SHA1))
-  | ( 0xc0z, 0x12z ) -> Correct(CipherSuite Kex_ECDHE (Some RSASIG) (MtE (Block TDES_EDE_CBC) SHA1))
-  | ( 0xc0z, 0x13z ) -> Correct(CipherSuite Kex_ECDHE (Some RSASIG) (MtE (Block AES_128_CBC) SHA1))
-  | ( 0xc0z, 0x14z ) -> Correct(CipherSuite Kex_ECDHE (Some RSASIG) (MtE (Block AES_256_CBC) SHA1))
-  | ( 0xc0z, 0x27z ) -> Correct(CipherSuite Kex_ECDHE (Some RSASIG) (MtE (Block AES_128_CBC) SHA256))
-  | ( 0xc0z, 0x28z ) -> Correct(CipherSuite Kex_ECDHE (Some RSASIG) (MtE (Block AES_256_CBC) SHA384))
-
-  (**************************************************************************)
-  | ( 0xc0z, 0x2bz ) -> Correct(CipherSuite Kex_ECDHE (Some ECDSA) (AEAD AES_128_GCM SHA256))
-  | ( 0xc0z, 0x2fz ) -> Correct(CipherSuite Kex_ECDHE (Some RSASIG) (AEAD AES_128_GCM SHA256))
-  | ( 0xc0z, 0x2cz ) -> Correct(CipherSuite Kex_ECDHE (Some ECDSA) (AEAD AES_256_GCM SHA384))
-  | ( 0xc0z, 0x30z ) -> Correct(CipherSuite Kex_ECDHE (Some RSASIG) (AEAD AES_256_GCM SHA384))
-
-  (**************************************************************************)
-  | ( 0xd0z, 0x01z ) -> Correct(CipherSuite Kex_PSK_ECDHE None (AEAD AES_128_GCM SHA256))
-  | ( 0xd0z, 0x02z ) -> Correct(CipherSuite Kex_PSK_ECDHE None (AEAD AES_256_GCM SHA384))
-
-  (**************************************************************************)
-  | ( 0x00z, 0x18z ) -> Correct(CipherSuite Kex_DHE None (MtE (Stream RC4_128) MD5))
-  | ( 0x00z, 0x1Bz ) -> Correct(CipherSuite Kex_DHE None (MtE (Block TDES_EDE_CBC) SHA1))
-  | ( 0x00z, 0x34z ) -> Correct(CipherSuite Kex_DHE None (MtE (Block AES_128_CBC) SHA1))
-  | ( 0x00z, 0x3Az ) -> Correct(CipherSuite Kex_DHE None (MtE (Block AES_256_CBC) SHA1))
-  | ( 0x00z, 0x6Cz ) -> Correct(CipherSuite Kex_DHE None (MtE (Block AES_128_CBC) SHA256))
-  | ( 0x00z, 0x6Dz ) -> Correct(CipherSuite Kex_DHE None (MtE (Block AES_256_CBC) SHA256))
-
-  (**************************************************************************)
-  | ( 0x00z, 0x9Cz ) -> Correct(CipherSuite Kex_RSA None (AEAD AES_128_GCM SHA256))
-  | ( 0x00z, 0x9Dz ) -> Correct(CipherSuite Kex_RSA None (AEAD AES_256_GCM SHA384))
-
-  | ( 0x00z, 0x9Ez ) -> Correct(CipherSuite Kex_DHE (Some RSASIG) (AEAD AES_128_GCM SHA256))
-  | ( 0x00z, 0x9Fz ) -> Correct(CipherSuite Kex_DHE (Some RSASIG) (AEAD AES_256_GCM SHA384))
-  | ( 0x00z, 0xA0z ) -> Correct(CipherSuite Kex_DH (Some RSASIG)  (AEAD AES_128_GCM SHA256))
-  | ( 0x00z, 0xA1z ) -> Correct(CipherSuite Kex_DH (Some RSASIG)  (AEAD AES_256_GCM SHA384))
-
-  | ( 0x00z, 0xA2z ) -> Correct(CipherSuite Kex_DHE (Some DSA) (AEAD AES_128_GCM SHA256))
-  | ( 0x00z, 0xA3z ) -> Correct(CipherSuite Kex_DHE (Some DSA) (AEAD AES_256_GCM SHA384))
-  | ( 0x00z, 0xA4z ) -> Correct(CipherSuite Kex_DH (Some DSA)  (AEAD AES_128_GCM SHA256))
-  | ( 0x00z, 0xA5z ) -> Correct(CipherSuite Kex_DH (Some DSA)  (AEAD AES_256_GCM SHA384))
-
-  | ( 0x00z, 0xA6z ) -> Correct(CipherSuite Kex_DHE None (AEAD AES_128_GCM SHA256))
-  | ( 0x00z, 0xA7z ) -> Correct(CipherSuite Kex_DHE None (AEAD AES_256_GCM SHA384))
-
-  (**************************************************************************)
-  | ( 0x00z, 0xaaz ) -> Correct(CipherSuite Kex_PSK_DHE None (AEAD AES_128_GCM SHA256))
-  | ( 0x00z, 0xabz ) -> Correct(CipherSuite Kex_PSK_DHE None (AEAD AES_256_GCM SHA384))
-
-  (**************************************************************************)
-  | ( 0x00z, 0xFFz ) -> Correct(SCSV (TLS_EMPTY_RENEGOTIATION_INFO_SCSV))
-  | (b1, b2) -> Correct(UnknownCipherSuite b1 b2)
-// Was:  | _ -> Error(AD_decode_error, perror __SOURCE_FILE__ __LINE__ "Parsed unknown cipher")
-
-(** Parsing function for ciphersuites *)
-val parseCipherSuite: pinverse_t cipherSuiteBytes
-let parseCipherSuite b =
-  match parseCipherSuiteAux b with
-  | Correct c -> Correct c
-  | Error z -> Error z
-
-
-#reset-options "--z3rlimit 60 --max_ifuel 6 --initial_ifuel 6 --max_fuel 1 --initial_fuel 1"
-
-(** Lemma for ciphersuite serializing/parsing inversions *)
-val inverse_cipherSuite: x:cipherSuite -> Lemma
-  (requires (~ (is_UnknownCipherSuite x)))
-  // parse (bytes (Unknown 0 0)) = NullCiphersuite
-  // must exclude this case...
-  (ensures (let y = cipherSuiteBytesOpt x in
-	(is_Some y ==> parseCipherSuiteAux (Some.v y) = Correct x)))
-  [SMTPat (parseCipherSuiteAux (Some.v (cipherSuiteBytesOpt x)))]
-let inverse_cipherSuite x = ()
-
-(** Lemma for ciphersuite serializing/parsing inversions *)
-val pinverse_cipherSuite : x:lbytes 2 -> Lemma
-  (requires (True))
-  (ensures (let y = parseCipherSuiteAux x in
-	    (is_Correct y ==>
-              (if is_UnknownCipherSuite (Correct._0 y) then true
-              else is_Some (cipherSuiteBytesOpt (Correct._0 y))
-               /\ Seq.equal x (Some.v (cipherSuiteBytesOpt (Correct._0 y)))))))
-  [SMTPat (cipherSuiteBytesOpt (Correct._0 (parseCipherSuiteAux x)))]
-let pinverse_cipherSuite x = ()
-
-
-#reset-options
-#set-options "--max_ifuel 1 --initial_ifuel 1 --max_fuel 1 --initial_fuel 1"
-
-(** Serializing function for a list of ciphersuite *)
-val cipherSuitesBytes: css:list (c:cipherSuite{validCipherSuite c}) -> Tot (lbytes (op_Multiply 2 (List.Tot.length css)))
-let rec cipherSuitesBytes css =
-  match css with
-  | [] -> empty_bytes
-  | cs::css -> (cipherSuiteBytes cs) @| (cipherSuitesBytes css)
-
-// Called by the server handshake;
-// ciphersuites that we do not understand are parsed, but ignored
-
-(** Parsing function for a list of ciphersuites *)
-val parseCipherSuites: b:bytes -> Tot (result (list (c:cipherSuite{validCipherSuite c}))) (decreases (length b))
-let rec parseCipherSuites b =
-  if length b > 1 then
-    let (b0,b1) = split b 2 in
-    match parseCipherSuites b1 with
-      | Correct(css) ->
-	(match parseCipherSuite b0 with
-	 | Error z ->	Correct css
-	 | Correct cs -> Correct (cs::css))
-      | Error z -> Error z
-  else
-  if length b = 0 then Correct []
-  else Error(AD_decode_error, perror __SOURCE_FILE__ __LINE__ "Odd cs bytes number")
-
-
-#reset-options
-#set-options "--max_ifuel 2 --initial_ifuel 2 --max_fuel 2 --initial_fuel 2"
-
-(** Lemma for ciphersuite lists serializing/parsing inversions *)
-val inverse_cipherSuites: x:list (c:cipherSuite{validCipherSuite c}) -> Lemma
-  (requires (true))
-  (ensures (parseCipherSuites (cipherSuitesBytes x) = Correct x))
-  [SMTPat (parseCipherSuites (cipherSuitesBytes x))]
-let rec inverse_cipherSuites x =
-  match x with
-  | [] -> ()
-  | cs::css ->
-     assume (~ (is_UnknownCipherSuite cs)); // TODO enforce it
-     let b = (cipherSuiteBytes cs) @| (cipherSuitesBytes css) in
-     let (b0,b1) = split b 2 in
-     lemma_append_inj b0 b1 (cipherSuiteBytes cs) (cipherSuitesBytes css);
-     inverse_cipherSuite cs;
-     inverse_cipherSuites css
-
-// REMARK: cipherSuitesBytes is not a partial inverse of parseCipherSuites,
-// because parseCipherSuites drops unknown ciphersuites.
-// Alternatively, we could add an UNKNOWN of (lbyte 2) constructor in cipherSuite
-// to make this hold.
-//
-// TODO: We added such constructor, so this is the case now. Prove it.
-
 
 (** Determine if a ciphersuite implies no peer authentication *)
 let isAnonCipherSuite cs =
@@ -920,6 +444,79 @@ type cipherSuiteName =
   | TLS_DH_anon_WITH_AES_256_GCM_SHA384
 
 
+val known_cipher_suite: cipherSuite -> Tot bool 
+let known_cipher_suite cs =
+    match cs with
+    | UnknownCipherSuite _ _
+    | NullCipherSuite          
+    | CipherSuite Kex_RSA None (MACOnly MD5) 
+    | CipherSuite Kex_RSA None (MACOnly SHA1)
+    | CipherSuite Kex_RSA None (MACOnly SHA256)
+    | CipherSuite Kex_RSA None(MtE (Stream RC4_128) MD5)
+    | CipherSuite Kex_RSA None(MtE (Stream RC4_128) SHA1)
+    | CipherSuite Kex_RSA None(MtE (Block TDES_EDE_CBC) SHA1)  
+    | CipherSuite Kex_RSA None(MtE (Block AES_128_CBC) SHA1)   
+    | CipherSuite Kex_RSA None(MtE (Block AES_256_CBC) SHA1)   
+    | CipherSuite Kex_RSA None(MtE (Block AES_128_CBC) SHA256) 
+    | CipherSuite Kex_RSA None(MtE (Block AES_256_CBC) SHA256) 
+    | CipherSuite Kex_DH (Some DSA)     (MtE (Block TDES_EDE_CBC) SHA1)  
+    | CipherSuite Kex_DH (Some RSASIG)  (MtE (Block TDES_EDE_CBC) SHA1)  
+    | CipherSuite Kex_DHE (Some DSA)    (MtE (Block TDES_EDE_CBC) SHA1)  
+    | CipherSuite Kex_DHE (Some RSASIG) (MtE (Block TDES_EDE_CBC) SHA1)  
+    | CipherSuite Kex_DH (Some DSA)     (MtE (Block AES_128_CBC) SHA1)   
+    | CipherSuite Kex_DH (Some RSASIG)  (MtE (Block AES_128_CBC) SHA1)   
+    | CipherSuite Kex_DHE (Some DSA)    (MtE (Block AES_128_CBC) SHA1)   
+    | CipherSuite Kex_DHE (Some RSASIG) (MtE (Block AES_128_CBC) SHA1)   
+    | CipherSuite Kex_DH (Some DSA)     (MtE (Block AES_256_CBC) SHA1)   
+    | CipherSuite Kex_DH (Some RSASIG)  (MtE (Block AES_256_CBC) SHA1)   
+    | CipherSuite Kex_DHE (Some DSA)    (MtE (Block AES_256_CBC) SHA1)   
+    | CipherSuite Kex_DHE (Some RSASIG) (MtE (Block AES_256_CBC) SHA1)   
+    | CipherSuite Kex_DH (Some DSA)     (MtE (Block AES_128_CBC) SHA256) 
+    | CipherSuite Kex_DH (Some RSASIG)  (MtE (Block AES_128_CBC) SHA256) 
+    | CipherSuite Kex_DHE (Some DSA)    (MtE (Block AES_128_CBC) SHA256) 
+    | CipherSuite Kex_DHE (Some RSASIG) (MtE (Block AES_128_CBC) SHA256) 
+    | CipherSuite Kex_DH (Some DSA)     (MtE (Block AES_256_CBC) SHA256) 
+    | CipherSuite Kex_DH (Some RSASIG)  (MtE (Block AES_256_CBC) SHA256) 
+    | CipherSuite Kex_DHE (Some DSA)    (MtE (Block AES_256_CBC) SHA256) 
+    | CipherSuite Kex_DHE (Some RSASIG) (MtE (Block AES_256_CBC) SHA256) 
+    | CipherSuite Kex_ECDHE (Some RSASIG) (MtE (Stream RC4_128) SHA1)      
+    | CipherSuite Kex_ECDHE (Some RSASIG) (MtE (Block TDES_EDE_CBC) SHA1)  
+    | CipherSuite Kex_ECDHE (Some RSASIG) (MtE (Block AES_128_CBC) SHA1)   
+    | CipherSuite Kex_ECDHE (Some RSASIG) (MtE (Block AES_256_CBC) SHA1)   
+    | CipherSuite Kex_ECDHE (Some RSASIG) (MtE (Block AES_128_CBC) SHA256) 
+    | CipherSuite Kex_ECDHE (Some RSASIG) (MtE (Block AES_256_CBC) SHA384) 
+    | CipherSuite Kex_ECDHE (Some RSASIG) (AEAD AES_128_GCM SHA256)
+    | CipherSuite Kex_ECDHE (Some ECDSA)  (AEAD AES_128_GCM SHA256)
+    | CipherSuite Kex_ECDHE (Some RSASIG) (AEAD AES_256_GCM SHA384)
+    | CipherSuite Kex_ECDHE (Some ECDSA) (AEAD AES_256_GCM SHA384) 
+    | CipherSuite Kex_PSK_DHE None (AEAD AES_128_GCM SHA256) 
+    | CipherSuite Kex_PSK_DHE None (AEAD AES_256_GCM SHA384) 
+    | CipherSuite Kex_PSK_ECDHE None (AEAD AES_128_GCM SHA256)
+    | CipherSuite Kex_PSK_ECDHE None (AEAD AES_256_GCM SHA384)
+    | CipherSuite Kex_DHE None   (MtE (Stream RC4_128) MD5)       
+    | CipherSuite Kex_DHE None   (MtE (Block TDES_EDE_CBC) SHA1)  
+    | CipherSuite Kex_DHE None   (MtE (Block AES_128_CBC) SHA1)   
+    | CipherSuite Kex_DHE None   (MtE (Block AES_256_CBC) SHA1)   
+    | CipherSuite Kex_DHE None   (MtE (Block AES_128_CBC) SHA256) 
+    | CipherSuite Kex_DHE None   (MtE (Block AES_256_CBC) SHA256) 
+    | CipherSuite Kex_RSA None     (AEAD AES_128_GCM SHA256) 
+    | CipherSuite Kex_RSA None     (AEAD AES_256_GCM SHA384) 
+    | CipherSuite Kex_DHE (Some RSASIG) (AEAD AES_128_GCM SHA256)
+    | CipherSuite Kex_DHE (Some RSASIG) (AEAD AES_256_GCM SHA384)
+    | CipherSuite Kex_DH (Some RSASIG)  (AEAD AES_128_GCM SHA256)
+    | CipherSuite Kex_DH (Some RSASIG)  (AEAD AES_256_GCM SHA384)
+    | CipherSuite Kex_DHE (Some DSA) (AEAD AES_128_GCM SHA256)
+    | CipherSuite Kex_DHE (Some DSA) (AEAD AES_256_GCM SHA384)
+    | CipherSuite Kex_DH (Some DSA)  (AEAD AES_128_GCM SHA256)
+    | CipherSuite Kex_DH (Some DSA)  (AEAD AES_256_GCM SHA384)
+    | CipherSuite Kex_DHE None (AEAD AES_128_GCM SHA256)
+    | CipherSuite Kex_DHE None (AEAD AES_256_GCM SHA384)
+    | SCSV (TLS_EMPTY_RENEGOTIATION_INFO_SCSV)        -> true
+    | _ -> false
+
+type valid_cipher_suite = c:cipherSuite{known_cipher_suite c}
+type valid_cipher_suites = list valid_cipher_suite
+
 (** Definition of a list of ciphersuite *)
 type cipherSuiteNames = list cipherSuiteName
 
@@ -1072,82 +669,9 @@ let rec names_of_cipherSuites css =
       end
     end
 
-// Note:
-// Migrated contentType to Content.fst (this is internal to TLS)
 
-(** Transforms a sequence of natural numbers into bytes *)
-val bytes_of_seq: n:nat{ repr_bytes n <= 8 } -> Tot bytes
-let bytes_of_seq sn = bytes_of_int 8 sn
-
-(** Transforms bytes into a sequence of natural numbers *)
-val seq_of_bytes: b:bytes{ length b <= 8 } -> Tot nat
-let seq_of_bytes b = int_of_bytes b
-
-(** Transform and concatenate a natural number to bytes *)
-val vlbytes: lSize:nat -> b:bytes{repr_bytes (length b) <= lSize} -> Tot (r:bytes{length r = lSize + length b})
-let vlbytes lSize b = bytes_of_int lSize (length b) @| b
-
-(** Lemmas associated to bytes manipulations *)
-val lemma_vlbytes_len : i:nat -> b:bytes{repr_bytes (length b) <= i}
-  -> Lemma (ensures (length (vlbytes i b) = i + length b))
-let lemma_vlbytes_len i b = ()
-
-val lemma_vlbytes_inj : i:nat
-  -> b:bytes{repr_bytes (length b) <= i}
-  -> b':bytes{repr_bytes (length b') <= i}
-  -> Lemma (requires (Seq.equal (vlbytes i b) (vlbytes i b')))
-          (ensures (b == b'))
-let lemma_vlbytes_inj i b b' =
-  let l = bytes_of_int i (length b) in
-  SeqProperties.lemma_append_inj l b l b'
-
-val vlbytes_length_lemma: n:nat -> a:bytes{repr_bytes (length a) <= n} -> b:bytes{repr_bytes (length b) <= n} -> 
-  Lemma (requires (Seq.equal (Seq.slice (vlbytes n a) 0 n) (Seq.slice (vlbytes n b) 0 n)))
-        (ensures (length a = length b))
-let vlbytes_length_lemma n a b = 
-  let lena = Seq.slice (vlbytes n a) 0 n in
-  let lenb = Seq.slice (vlbytes n b) 0 n in
-  assert(Seq.equal lena (bytes_of_int n (length a)));
-  assert(Seq.equal lenb (bytes_of_int n (length b)));
-  int_of_bytes_of_int n (length a); int_of_bytes_of_int n (length b)
-
-
-#set-options "--max_ifuel 1 --initial_ifuel 1 --max_fuel 0 --initial_fuel 0"   //need to reason about length
-
-
-val vlsplit: lSize:nat{lSize <= 4}
-  -> vlb:bytes{lSize <= length vlb}
-  -> Tot (result (b:(bytes * bytes){
-                    repr_bytes (length (fst b)) <= lSize
-                  /\ Seq.equal vlb (vlbytes lSize (fst b) @| (snd b))}))
-let vlsplit lSize vlb =
-  let (vl,b) = Platform.Bytes.split vlb lSize in
-  let l = int_of_bytes vl in
-  if l <= length b
-  then Correct(Platform.Bytes.split b l)
-  else Error(AD_decode_error, perror __SOURCE_FILE__ __LINE__ "")
-
-
-val vlparse: lSize:nat{lSize <= 4} -> vlb:bytes{lSize <= length vlb}
-  -> Tot (result (b:bytes{repr_bytes (length b) <= lSize /\ Seq.equal vlb (vlbytes lSize b)}))
-let vlparse lSize vlb =
-  let vl,b = split vlb lSize in
-  if int_of_bytes vl = length b
-  then Correct b
-  else Error(AD_decode_error, perror __SOURCE_FILE__ __LINE__ "")
-
-
-val vlparse_vlbytes: lSize:nat{lSize <= 4} -> vlb:bytes{repr_bytes (length vlb) <= lSize} -> Lemma 
-  (requires (True))
-  (ensures (vlparse lSize (vlbytes lSize vlb) == Correct vlb))
-  [SMTPat (vlparse lSize (vlbytes lSize vlb))]
-let vlparse_vlbytes lSize vlb =
-  let vl,b = split (vlbytes lSize vlb) lSize in
-  assert (Seq.equal vl (bytes_of_int lSize (length vlb)));
-  int_of_bytes_of_int lSize (length vlb);
-  match vlparse lSize (vlbytes lSize vlb) with
-  | Error z   -> ()
-  | Correct b -> lemma_vlbytes_inj lSize vlb b
+type cert = b:bytes {length b <= 16777215}
+type chain = list cert
 
 
 (** Certificate type definition *)
@@ -1156,65 +680,6 @@ type certType =
   | DSA_sign
   | RSA_fixed_dh
   | DSA_fixed_dh
-
-(** Serializing function for the certificate type *)
-val certTypeBytes: certType -> Tot (lbytes 1)
-let certTypeBytes ct =
-  match ct with
-  | RSA_sign     -> abyte 1z
-  | DSA_sign     -> abyte 2z
-  | RSA_fixed_dh -> abyte 3z
-  | DSA_fixed_dh -> abyte 4z
-
-(** Parsing function for the certificate type *)
-val parseCertType: pinverse_t certTypeBytes
-let parseCertType b =
-  match cbyte b with
-  | 1z -> Correct RSA_sign
-  | 2z -> Correct DSA_sign
-  | 3z -> Correct RSA_fixed_dh
-  | 4z -> Correct DSA_fixed_dh
-  | _ -> Error(AD_decode_error, perror __SOURCE_FILE__ __LINE__ "")
-
-
-(** Lemmas associated to serializing/parsing of certificate types *)
-val inverse_certType: x:_ -> Lemma
-  (requires (True))
-  (ensures lemma_inverse_g_f certTypeBytes parseCertType x)
-  [SMTPat (parseCertType (certTypeBytes x))]
-let inverse_certType x = ()
-
-val pinverse_certType: x:_ -> Lemma
-  (requires (True))
-  (ensures (lemma_pinverse_f_g Seq.equal certTypeBytes parseCertType x))
-  [SMTPat (certTypeBytes (Correct._0 (parseCertType x)))]
-let pinverse_certType x = ()
-
-
-#set-options "--max_fuel 1 --initial_fuel 1"
-
-(** Serializing function for lists of certificate types *)
-val certificateTypeListBytes: ctl:list certType -> Tot (lbytes (List.Tot.length ctl))
-let rec certificateTypeListBytes ctl =
-  match ctl with
-  | [] -> empty_bytes
-  | h::t ->
-    let ct = certTypeBytes h in
-    ct @| certificateTypeListBytes t
-
-(** Parsing function for lists of certificate types *)
-val parseCertificateTypeList: data:bytes -> Tot (list certType) (decreases (length data))
-let rec parseCertificateTypeList data =
-  if length data = 0 then []
-  else
-    let (thisByte,data) = Platform.Bytes.split data 1 in
-    match parseCertType thisByte with
-    | Error z -> // we skip this one
-      parseCertificateTypeList data
-    | Correct ct ->
-      let rem = parseCertificateTypeList data in
-      ct :: rem
-
 
 #set-options "--max_ifuel 4 --initial_ifuel 1 --max_fuel 4 --initial_fuel 1"
 
@@ -1240,38 +705,6 @@ let defaultCertTypes sign cs =
 
 (** Type definition of the Distinguished Name of a certificate *)
 type dn = s:string{length(utf8 s) <= 256}
-
-(** Serializing function for a list of Distinguished Names of certificates *)
-val distinguishedNameListBytes: names:list dn -> Tot (b:bytes{length b <= op_Multiply 258 (List.Tot.length names)})
-let rec distinguishedNameListBytes names =
-  match names with
-  | [] -> empty_bytes
-  | h::t ->
-    lemma_repr_bytes_values (length (utf8 h));
-    let name = vlbytes 2 (utf8 h) in
-    name @| distinguishedNameListBytes t
-
-(** Parsing function for a list of Distinguished Names of certificates *)
-val parseDistinguishedNameList: data:bytes -> res:list dn -> Tot (result (list dn)) (decreases (length data))
-let rec parseDistinguishedNameList data res =
-  if length data = 0 then
-    Correct res
-  else
-    if length data < 2 then
-      Error(AD_decode_error, perror __SOURCE_FILE__ __LINE__ "")
-    else
-      match vlsplit 2 data with
-      | Error z -> Error z
-      | Correct (nameBytes,data) ->
-        begin
-	match iutf8_opt nameBytes with
-        | None -> Error(AD_decode_error, perror __SOURCE_FILE__ __LINE__ "")
-        | Some name ->
-	  if length (utf8 name) < 256 then
-          let res = name :: res in
-          parseDistinguishedNameList data res
-	  else Error(AD_decode_error, perror __SOURCE_FILE__ __LINE__ "")
-        end
 
 (** Determine if a ciphersuite list contains the SCSV ciphersuite *)
 let contains_TLS_EMPTY_RENEGOTIATION_INFO_SCSV (css: list cipherSuite) =
@@ -1304,166 +737,8 @@ type namedGroup =
   | FFDHE_PRIVATE_USE of (b:byte{b = 0xFCz \/ b = 0xFDz \/ b = 0xFEz \/ b = _FFz})
   | ECDHE_PRIVATE_USE of byte
 
-(** Serializing function for (EC)DHE named groups *)
-val namedGroupBytes: namedGroup -> Tot (lbytes 2)
-let namedGroupBytes ng =
-  match ng with
-  | SEC ec ->
-    begin
-    match ec with
-    | ECC_P256		-> abyte2 (0x00z, 0x17z)
-    | ECC_P384		-> abyte2 (0x00z, 0x18z)
-    | ECC_P521		-> abyte2 (0x00z, 0x19z)
-    end
-  | EC_UNSUPPORTED b	-> abyte2 (0x00z, b)
-  | FFDHE dhe ->
-    begin
-    match dhe with
-    | FFDHE2048		-> abyte2 (0x01z, 0x00z)
-    | FFDHE3072		-> abyte2 (0x01z, 0x01z)
-    | FFDHE4096		-> abyte2 (0x01z, 0x02z)
-    | FFDHE6144		-> abyte2 (0x01z, 0x03z)
-    | FFDHE8192		-> abyte2 (0x01z, 0x04z)
-    end
-  | FFDHE_PRIVATE_USE b -> abyte2 (0x01z, b)
-  | ECDHE_PRIVATE_USE b -> abyte2 (0xFEz, b)
-
-(** Parsing function for (EC)DHE named groups *)
-val parseNamedGroup: pinverse_t namedGroupBytes
-let parseNamedGroup b =
-  match cbyte2 b with
-  | (0x00z, 0x17z) -> Correct (SEC ECC_P256)
-  | (0x00z, 0x18z) -> Correct (SEC ECC_P384)
-  | (0x00z, 0x19z) -> Correct (SEC ECC_P521)
-  | (0x00z, b)     -> Correct (EC_UNSUPPORTED b) // REMARK: only values 0x01z-0x16z and 0x1Az-0x1Ez are assigned
-  | (0x01z, 0x00z) -> Correct (FFDHE FFDHE2048)
-  | (0x01z, 0x01z) -> Correct (FFDHE FFDHE3072)
-  | (0x01z, 0x02z) -> Correct (FFDHE FFDHE4096)
-  | (0x01z, 0x03z) -> Correct (FFDHE FFDHE6144)
-  | (0x01z, 0x04z) -> Correct (FFDHE FFDHE8192)
-  | (0x01z, b)     ->
-    if b = 0xFCz || b = 0xFDz || b = 0xFEz || b = 0xFFz
-    then Correct (FFDHE_PRIVATE_USE b)
-    else Error (AD_decode_error, perror __SOURCE_FILE__ __LINE__ "Wrong ffdhe private use group")
-  | (0xFEz, b)     -> Correct (ECDHE_PRIVATE_USE b)
-  | _ -> Error (AD_decode_error, perror __SOURCE_FILE__ __LINE__ "Wrong named group")
-
-(** Lemmas for named groups parsing/serializing inversions *)
-val inverse_namedGroup: x:_ -> Lemma
-  (requires (True))
-  (ensures lemma_inverse_g_f namedGroupBytes parseNamedGroup x)
-  [SMTPat (parseNamedGroup (namedGroupBytes x))]
-let inverse_namedGroup x = ()
-
-val pinverse_namedGroup: x:_ -> Lemma
-  (requires (True))
-  (ensures (lemma_pinverse_f_g Seq.equal namedGroupBytes parseNamedGroup x))
-  [SMTPat (namedGroupBytes (Correct._0 (parseNamedGroup x)))]
-let pinverse_namedGroup x = ()
-
-
-private val namedGroupsBytes0: groups:list namedGroup
-  -> Tot (b:bytes { length b = op_Multiply 2 (List.Tot.length groups)})
-let rec namedGroupsBytes0 groups =
-  match groups with
-  | [] -> empty_bytes
-  | g::gs -> namedGroupBytes g @| namedGroupsBytes0 gs
-
-(** Serialization function for a list of named groups *)
-val namedGroupsBytes: groups:list namedGroup{List.Tot.length groups < 65536/2}
-  -> Tot (b:bytes { length b = 2 + op_Multiply 2 (List.Tot.length groups)})
-let namedGroupsBytes groups =
-  let gs = namedGroupsBytes0 groups in
-  lemma_repr_bytes_values (length gs);
-  vlbytes 2 gs
-
-private val parseNamedGroups0: b:bytes -> l:list namedGroup
-  -> Tot (result (groups:list namedGroup{List.Tot.length groups = List.Tot.length l + length b / 2}))
-  (decreases (length b))
-let rec parseNamedGroups0 b groups =
-  if length b > 0 then
-    if length b >= 2 then
-      let (ng, bytes) = split b 2 in
-      lemma_split b 2;
-      match parseNamedGroup ng with
-      |Correct ng ->
-        let groups' = ng :: groups in
-        parseNamedGroups0 bytes groups'
-      | Error z    -> Error z
-    else Error (AD_decode_error, perror __SOURCE_FILE__ __LINE__ "")
-  else
-   let grev = List.Tot.rev groups in
-   assume (List.Tot.length grev == List.Tot.length groups);
-   Correct grev
-
-(** Parsing function for a list of named groups *)
-val parseNamedGroups: b:bytes { 2 <= length b /\ length b < 65538 }
-  -> Tot (result (groups:list namedGroup{List.Tot.length groups = (length b - 2) / 2}))
-let parseNamedGroups b =
-  match vlparse 2 b with
-  | Correct b -> parseNamedGroups0 b []
-  | Error z   ->
-    Error(AD_decode_error, perror __SOURCE_FILE__ __LINE__ "Failed to parse named groups")
-
-
 (** Definition of the configuration identifier *)
 type configurationId = b:bytes{0 < length b /\ length b < 65536}
-
-(** Serializing function for the configuration identifier *)
-val configurationIdBytes: configurationId -> Tot (b:bytes{2 < length b /\ length b < 65538})
-let configurationIdBytes cid =
-  lemma_repr_bytes_values (length cid);
-  vlbytes 2 cid
-
-(** Parsing function for the configuration identifier *)
-val parseConfigurationId: pinverse_t configurationIdBytes
-let parseConfigurationId b =
-  match vlparse 2 b with
-  | Error z -> Error z
-  | Correct b -> Correct b
-
-(** Lemmas for configurationId serializing/parsing inversion *)
-val inverse_configurationId: x:_ -> Lemma
-  (requires (True))
-  (ensures lemma_inverse_g_f configurationIdBytes parseConfigurationId x)
-  [SMTPat (parseConfigurationId (configurationIdBytes x))]
-let inverse_configurationId x =
-  lemma_repr_bytes_values (length x)
-
-val pinverse_configurationId: x:_ -> Lemma
-  (requires (True))
-  (ensures (lemma_pinverse_f_g Seq.equal configurationIdBytes parseConfigurationId x))
-  [SMTPat (configurationIdBytes (Correct._0 (parseConfigurationId x)))]
-let pinverse_configurationId x = ()
-
-
-//
-// BB.TODO: Some of the following code should be moved outside TLSConstants !
-//          In particular, the integer definitions can be taken from F* ulib.
-
-type uint32 = b:lbytes 4
-
-val uint32Bytes: uint32 -> Tot (lbytes 4)
-let uint32Bytes u = u
-
-val parseUint32: pinverse_t uint32Bytes
-let parseUint32 b =
-  if length b = 4 then Correct(b)
-  else Error (AD_decode_error, perror __SOURCE_FILE__ __LINE__ "")
-
-val inverse_uint32: x:_ -> Lemma
-  (requires (True))
-  (ensures lemma_inverse_g_f uint32Bytes parseUint32 x)
-  [SMTPat (parseUint32 (uint32Bytes x))]
-let inverse_uint32 x = ()
-
-val pinverse_uint32: x:_ -> Lemma
-  (requires (True))
-  (ensures (lemma_pinverse_f_g Seq.equal uint32Bytes parseUint32 x))
-  [SMTPat (uint32Bytes (Correct._0 (parseUint32 x)))]
-let pinverse_uint32 x = ()
-
-
 
 (** EarlyData type definition *)
 type earlyDataType =
@@ -1471,184 +746,21 @@ type earlyDataType =
   | EarlyData
   | ClientAuthenticationAndData
 
-(** Serializing function for Early Data values *)
-val earlyDataTypeBytes: earlyDataType -> Tot (lbytes 1)
-let earlyDataTypeBytes edt =
-  match edt with
-  | ClientAuthentication        -> abyte 1z
-  | EarlyData                   -> abyte 2z
-  | ClientAuthenticationAndData -> abyte 3z
-
-(** Parsing function for Early Data values *)
-val parseEarlyDataType: pinverse_t earlyDataTypeBytes
-let parseEarlyDataType b =
-  match cbyte b with
-  | 1z -> Correct ClientAuthentication
-  | 2z -> Correct EarlyData
-  | 3z -> Correct ClientAuthenticationAndData
-  | _  -> Error (AD_decode_error, perror __SOURCE_FILE__ __LINE__ "Failed to parse early data type")
-
-
-(** Lemmas for Early Data parsing/serializing inversions *)
-val inverse_earlyDataType: x:_ -> Lemma
-  (requires (True))
-  (ensures lemma_inverse_g_f earlyDataTypeBytes parseEarlyDataType x)
-  [SMTPat (parseEarlyDataType (earlyDataTypeBytes x))]
-let inverse_earlyDataType x = ()
-
-val pinverse_earlyDataType: x:_ -> Lemma
-  (requires (True))
-  (ensures (lemma_pinverse_f_g Seq.equal earlyDataTypeBytes parseEarlyDataType x))
-  [SMTPat (earlyDataTypeBytes (Correct._0 (parseEarlyDataType x)))]
-let pinverse_earlyDataType x = ()
-
-
 // TODO: replace with more precise types when available
 (** Configuration Extension definition *)
 noeq type configurationExtension =
   | UnknownConfigurationExtension:
       typ:lbytes 2 -> payload: bytes { repr_bytes (length payload) <= 2 } -> configurationExtension
 
-// TODO: Should we strengthen the result type to b:bytes{length b >= 4}?
-(** Serialization of the configuration extension values *)
-val configurationExtensionBytes: ce:configurationExtension -> Tot bytes
-let configurationExtensionBytes ce =
-  match ce with
-  | UnknownConfigurationExtension typ payload -> typ @| vlbytes 2 payload
-
-(** Parsing of the configuration extension values *)
-val parseConfigurationExtension: pinverse_t configurationExtensionBytes
-let parseConfigurationExtension b =
-  if length b >= 4 then
-    let (typ,payload) = split b 2 in
-    match vlparse 2 payload with
-    | Correct payload -> Correct (UnknownConfigurationExtension typ payload)
-    | Error z -> Error z
-  else Error (AD_decode_error, perror __SOURCE_FILE__ __LINE__ "Too few bytes to parse a configuration extension")
-
-
-(** Lemmas for Configuration Extension parsing/serializing inversions *)
-val inverse_configurationExtension: x:_ -> Lemma
-  (requires (True))
-  (ensures lemma_inverse_g_f configurationExtensionBytes parseConfigurationExtension x)
-  [SMTPat (parseConfigurationExtension (configurationExtensionBytes x))]
-let inverse_configurationExtension x =
-  match x with
-  | UnknownConfigurationExtension typ payload ->
-  let b = typ @| vlbytes 2 payload in
-  let b0,b1 = split b 2 in
-  let vl,b = split b1 2 in
-  vlparse_vlbytes 2 b;
-  assert (Seq.equal vl (bytes_of_int 2 (length b)));
-  assert (Seq.equal b0 typ);
-  assert (Seq.equal b payload)
-
-val pinverse_configurationExtension: x:_ -> Lemma
-  (requires (True))
-  (ensures (lemma_pinverse_f_g Seq.equal configurationExtensionBytes parseConfigurationExtension x))
-  [SMTPat (configurationExtensionBytes (Correct._0 (parseConfigurationExtension x)))]
-let pinverse_configurationExtension x = ()
-
-
-// TODO: Choice, truncate when maximum length is exceeded
-(** Serialization of the configuration extension list of values *)
-val configurationExtensionsBytes: list configurationExtension -> Tot bytes
-let configurationExtensionsBytes ce =
-  let rec configurationExtensionsBytes_aux (b:bytes{length b < 65536}) (ces:list configurationExtension): Tot (b:bytes{length b < 65536}) (decreases ces) =
-  match ces with
-  | [] -> b
-  | ce::ces ->
-    if length (b @| configurationExtensionBytes ce) < 65536 then
-      configurationExtensionsBytes_aux (b @| configurationExtensionBytes ce) ces
-    else b
-  in
-  let b = configurationExtensionsBytes_aux empty_bytes ce in
-  lemma_repr_bytes_values (length b);
-  vlbytes 2 b
-
-(** Parsing of the configuration extension list of values *)
-val parseConfigurationExtensions: pinverse_t configurationExtensionsBytes
-let parseConfigurationExtensions b =
-  let rec (aux: b:bytes -> list configurationExtension -> Tot (result (list configurationExtension)) (decreases (length b))) =
-    fun b exts ->
-    if length b > 0 then
-      if length b >= 4 then
-	let typ, len, data = split2 b 2 2 in
-	let len = int_of_bytes len in
-	if length b >= 4 + len then
-	  let ext, bytes = split b len in
-	  match parseConfigurationExtension ext with
-	  | Correct(ext') -> aux bytes (ext'::exts)
-	  | Error(z) -> Error(z)
-	else Error(AD_decode_error, perror __SOURCE_FILE__ __LINE__ "Failed to parse configuration extension length")
-      else Error(AD_decode_error, perror __SOURCE_FILE__ __LINE__ "Configuration extension length should be at least 4")
-    else Correct(exts) in
-  if length b >= 2 then
-  match vlparse 2 b with
-  | Correct (b) ->  aux b []
-  | Error(z) -> Error(AD_decode_error, perror __SOURCE_FILE__ __LINE__ "Failed to parse configuration extension")
-  else Error(AD_decode_error, perror __SOURCE_FILE__ __LINE__ "Failed to parse configuration extension")
-
-
 (** Tuple Signature Algorithm and Hash Algorithm type definition *)
 type sigHashAlg = sigAlg * hashAlg'
-
-(** Serializing function for the Signature algorithm *)
-val sigHashAlgBytes: sigHashAlg -> Tot (lbytes 2)
-let sigHashAlgBytes sha =
-  let sign = sigAlgBytes (fst sha) in
-  let hash = hashAlgBytes (snd sha) in
-  hash @| sign
-
-(** Parsing function for the Signature algorithm *)
-val parseSigHashAlg: pinverse_t sigHashAlgBytes
-let parseSigHashAlg b =
-  let hash,sign = split b 1 in
-  match parseSigAlg sign with
-  | Correct sign ->
-    begin
-    match parseHashAlg hash with
-    | Correct hash -> Correct(sign, hash)
-    | Error z -> Error z
-    end
-  | Error z -> Error z
-
-// TODO: Moving this inside sigHashAlgsBytes gives a `Bound term variable not found` error
-// See https://github.com/FStarLang/FStar/issues/533
-
-(** Serializing function for a Signature algorithm list *)
-val sigHashAlgsBytes: algs:list sigHashAlg{List.Tot.length algs < 65536/2}
-  -> Tot (b:bytes{2 <= length b /\ length b < 65538})
-let sigHashAlgsBytes algs =
-  let rec sigHashAlgsBytes_aux: b:bytes
-    -> algs:list sigHashAlg{b2t (length b + op_Multiply 2 (List.Tot.length algs) < 65536)}
-    -> Tot (r:bytes{length r < 65536}) (decreases algs) = fun b algs ->
-    match algs with
-    | [] -> b
-    | alg::algs' ->
-      let shb = sigHashAlgBytes alg in
-      sigHashAlgsBytes_aux (shb @| b) algs'
-  in
-  let b = sigHashAlgsBytes_aux empty_bytes algs in
-  lemma_repr_bytes_values (length b);
-  vlbytes 2 b
-
-(** Parsing function for a Signature algorithm list *)
-val parseSigHashAlgs: pinverse_t sigHashAlgsBytes
-let parseSigHashAlgs b =
-  let rec aux: b:bytes -> algs:list sigHashAlg{length b + op_Multiply 2 (List.Tot.length algs) < 65536} -> Tot (result (l:list sigHashAlg{List.Tot.length l < 65536/2})) (decreases (length b)) = fun b algs ->
-    if length b > 0 then
-      if length b >= 2 then
-      let alg,bytes = split b 2 in
-      match parseSigHashAlg alg with
-      | Correct sha -> aux bytes (sha::algs)
-      | Error z     -> Error z
-      else Error (AD_decode_error, perror __SOURCE_FILE__ __LINE__ "Too few bytes to parse sig hash algs")
-    else Correct algs in
-  match vlparse 2 b with
-  | Correct b -> aux b []
-  | Error z   -> Error(AD_decode_error, perror __SOURCE_FILE__ __LINE__ "Failed to parse sig hash algs")
-
+type sigScheme = 
+  | SigHashAlg of sigHashAlg
+  | RSA_PSS_SHA256
+  | RSA_PSS_SHA384
+  | RSA_PSS_SHA512
+  | ED25519	
+  | ED448
 
 // TODO: replace "bytes" by either DH or ECDH parameters
 (** KeyShare entry definition *)
@@ -1666,194 +778,10 @@ noeq type keyShare =
   | ClientKeyShare of clientKeyShare
   | ServerKeyShare of serverKeyShare
 
-(** Serializing function for a KeyShareEntry *)
-val keyShareEntryBytes: keyShareEntry -> Tot (b:bytes{4 <= length b})
-let keyShareEntryBytes (ng, b) =
-  let ng_bytes = namedGroupBytes ng in
-  ng_bytes @| vlbytes 2 b
-
-(** Parsing function for a KeyShareEntry *)
-val parseKeyShareEntry: pinverse_t keyShareEntryBytes
-let parseKeyShareEntry b =
-  let ng,key_exchange = split b 2 in
-  match parseNamedGroup ng with
-  | Correct ng ->
-    begin
-    match vlparse 2 key_exchange with
-    | Correct ke -> Correct (ng, ke)
-    | Error z    -> Error(AD_decode_error, perror __SOURCE_FILE__ __LINE__ "Failed to parse key share entry")
-    end
-  | Error z -> Error z
-
-
-(** Lemmas for KeyShare entries parsing/serializing inversions *)
-val inverse_keyShareEntry: x:_ -> Lemma
-  (requires (True))
-  (ensures lemma_inverse_g_f keyShareEntryBytes parseKeyShareEntry x)
-  [SMTPat (parseKeyShareEntry (keyShareEntryBytes x))]
-let inverse_keyShareEntry (ng, x) =
-  let b = namedGroupBytes ng @| vlbytes 2 x in
-  let b0,b1 = split b 2 in
-  let vl,b = split b1 2 in
-  vlparse_vlbytes 2 b;
-  assert (Seq.equal vl (bytes_of_int 2 (length b)));
-  assert (Seq.equal b0 (namedGroupBytes ng));
-  assert (Seq.equal b x)
-
-val pinverse_keyShareEntry: x:_ -> Lemma
-  (requires (True))
-  (ensures lemma_pinverse_f_g Seq.equal keyShareEntryBytes parseKeyShareEntry x)
-  [SMTPat (keyShareEntryBytes (Correct._0 (parseKeyShareEntry x)))]
-let pinverse_keyShareEntry x = ()
-
-
-// Choice: truncate when maximum length is exceeded
-(** Serializing function for a list of KeyShareEntry *)
-val keyShareEntriesBytes: list keyShareEntry -> Tot (b:bytes{2 <= length b /\ length b < 65538})
-let keyShareEntriesBytes kes =
-  let rec keyShareEntriesBytes_aux (b:bytes{length b < 65536}) (kes:list keyShareEntry): Tot (b:bytes{length b < 65536}) (decreases kes) =
-  match kes with
-  | [] -> b
-  | ke::kes ->
-    let b' = b @| keyShareEntryBytes ke in
-    if length b' < 65536 then
-      keyShareEntriesBytes_aux b' kes
-    else b
-  in
-  let b = keyShareEntriesBytes_aux empty_bytes kes in
-  lemma_repr_bytes_values (length b);
-  vlbytes 2 b
-
-(** Parsing function for a list KeyShareEntry *)
-val parseKeyShareEntries: pinverse_t keyShareEntriesBytes
-let parseKeyShareEntries b =
-  let rec (aux: b:bytes -> list keyShareEntry -> Tot (result (list keyShareEntry)) (decreases (length b))) = fun b entries ->
-    if length b > 0 then
-      if length b >= 4 then
-	let ng, data = split b 2 in
-	match vlsplit 2 data with
-	| Correct(kex, bytes) ->
-	  begin
-	  match parseKeyShareEntry (ng @| vlbytes 2 kex) with
-	  | Correct entry -> aux bytes (entries @ [entry])
-	  | Error z -> Error z
-	  end
-	| Error z -> Error(AD_decode_error, perror __SOURCE_FILE__ __LINE__ "Failed to parse key share entry")
-      else Error (AD_decode_error, perror __SOURCE_FILE__ __LINE__ "Too few bytes to parse key share entries")
-    else Correct entries in
-  match vlparse 2 b with
-  | Correct b -> aux b []
-  | Error z   -> Error(AD_decode_error, perror __SOURCE_FILE__ __LINE__ "Failed to parse key share entries")
-
-(** Serializing function for a ClientKeyShare *)
-val clientKeyShareBytes: clientKeyShare -> Tot (b:bytes{ 2 <= length b /\ length b < 65538 })
-let clientKeyShareBytes cks = keyShareEntriesBytes cks
-
-(** Parsing function for a ClientKeyShare *)
-val parseClientKeyShare: b:bytes{ 2 <= length b /\ length b < 65538 }
-  -> Tot (result clientKeyShare)
-let parseClientKeyShare b =
-  match parseKeyShareEntries b with
-  | Correct kes ->
-    if List.Tot.length kes < 65536/4
-    then Correct kes
-    else Error(AD_decode_error, perror __SOURCE_FILE__ __LINE__ "Failed to parse client key share entries")
-  | Error z -> Error z
-
-(** Serializing function for a ServerKeyShare *)
-val serverKeyShareBytes: serverKeyShare -> Tot (b:bytes{ 4 <= length b })
-let serverKeyShareBytes sks = keyShareEntryBytes sks
-
-(** Parsing function for a ServerKeyShare *)
-val parseServerKeyShare: pinverse_t serverKeyShareBytes
-let parseServerKeyShare b = parseKeyShareEntry b
-
-(** Serializing function for a KeyShare *)
-val keyShareBytes: keyShare -> Tot bytes
-let keyShareBytes = function
-  | ClientKeyShare cks -> clientKeyShareBytes cks
-  | ServerKeyShare sks -> serverKeyShareBytes sks
-
-(** Parsing function for a KeyShare *)
-val parseKeyShare: bool -> bytes -> Tot (result keyShare)
-let parseKeyShare is_client b =
-  if is_client then
-    begin
-    if 2 <= length b && length b < 65538 then
-      begin
-      match parseClientKeyShare b with
-      | Correct kse -> Correct (ClientKeyShare kse)
-      | Error z -> Error z
-      end
-    else Error(AD_decode_error, perror __SOURCE_FILE__ __LINE__ "Failed to parse key share")
-    end
-  else
-    if 4 <= length b then
-      begin
-      match parseServerKeyShare b with
-      | Correct ks -> Correct (ServerKeyShare ks)
-      | Error z -> Error z
-      end
-    else Error(AD_decode_error, perror __SOURCE_FILE__ __LINE__ "Failed to parse key share")
-
 // TODO: give more precise type
 
 (** PSK Identity definition *)
 type pskIdentity = b:bytes{repr_bytes (length b) <= 2}
-
-(** Serializing function for a PSK Identity *)
-val pskIdentityBytes: pskIdentity -> Tot (b:bytes{length b >= 2})
-let pskIdentityBytes pski =
-  vlbytes 2 pski
-
-(** Parsing function for a PSK Identity *)
-val parsePskIdentity: pinverse_t pskIdentityBytes
-let parsePskIdentity b =
-  match vlparse 2 b with
-  | Correct vlb -> Correct vlb
-  | Error z -> Error(AD_decode_error, perror __SOURCE_FILE__ __LINE__ "Failed to parse psk_identity")
-
-
-// TODO: Choice, truncate when maximum length is exceeded
-
-(** Serializing function for a list of PSK Identity *)
-val pskIdentitiesBytes: list pskIdentity -> Tot (b:bytes{2 <= length b /\ length b < 65538})
-let pskIdentitiesBytes ids =
-  let rec pskIdentitiesBytes_aux (b:bytes{length b < 65536}) (ids:list pskIdentity): Tot (b:bytes{length b < 65536}) (decreases ids) =
-  match ids with
-  | [] -> b
-  | id::ids ->
-    let b' = b @| pskIdentityBytes id in
-    if length b' < 65536 then
-      pskIdentitiesBytes_aux b' ids
-    else b
-  in
-  let b = pskIdentitiesBytes_aux empty_bytes ids in
-  lemma_repr_bytes_values (length b);
-  vlbytes 2 b
-
-(** Parsing function for a list of PSK Identity *)
-val parsePskIdentities: pinverse_t pskIdentitiesBytes
-let parsePskIdentities b =
-  let rec (aux: b:bytes -> list pskIdentity -> Tot (result (list pskIdentity)) (decreases (length b))) = fun b ids ->
-    if length b > 0 then
-      if length b >= 2 then
-	let len, data = split b 2 in
-	let len = int_of_bytes len in
-	if length b >= len then
-	  let pski,bytes = split b len in
-	  if length pski >= 2 then
-   	    match parsePskIdentity pski with
-   	    | Correct id -> aux bytes (id::ids)
-   	    | Error z -> Error z
-	  else Error(AD_decode_error, perror __SOURCE_FILE__ __LINE__ "Failed to parse psk identity length")
-        else Error(AD_decode_error, perror __SOURCE_FILE__ __LINE__ "Failed to parse psk identity length")
-      else Error(AD_decode_error, perror __SOURCE_FILE__ __LINE__ "Expected psk identity to be at least 2 bytes long")
-    else Correct ids in
-  match vlparse 2 b with
-  | Correct b -> aux b []
-  | Error z   -> Error(AD_decode_error, perror __SOURCE_FILE__ __LINE__ "Failed to parse psk identities")
-
 
 (** Client list of PSK identities *)
 type clientPreSharedKey = l:list pskIdentity{List.Tot.length l >= 1 /\ List.Tot.length l < 65536/2}
@@ -1866,58 +794,3 @@ noeq type preSharedKey =
   | ClientPreSharedKey of clientPreSharedKey
   | ServerPreSharedKey of serverPreSharedKey
 
-(** Serializing function for ClientPreSharedKey *)
-val clientPreSharedKeyBytes: clientPreSharedKey -> Tot (b:bytes{ 2 <= length b /\ length b < 65538 })
-let clientPreSharedKeyBytes cpsk = pskIdentitiesBytes cpsk
-
-(** Parsing function for ClientPreSharedKey *)
-val parseClientPreSharedKey: b:bytes{ 2 <= length b /\ length b < 65538 }
-  -> Tot (result clientPreSharedKey)
-let parseClientPreSharedKey b =
-  match parsePskIdentities b with
-  | Correct ids ->
-    let l = List.Tot.length ids in
-    if 1 <= l && l < 65536/2
-    then Correct ids
-    else Error(AD_decode_error, perror __SOURCE_FILE__ __LINE__ "Failed to parse client psk identities")
-  | Error z -> Error z
-
-(** Serializing function for ServerPreSharedKey *)
-val serverPreSharedKeyBytes: serverPreSharedKey -> Tot (b:bytes{ 2 <= length b })
-let serverPreSharedKeyBytes cpsk = pskIdentityBytes cpsk
-
-(** Parsing function for ServerPreSharedKey *)
-val parseServerPreSharedKey: pinverse_t serverPreSharedKeyBytes
-let parseServerPreSharedKey b = parsePskIdentity b
-
-(** Serializing function for PreSharedKey *)
-val preSharedKeyBytes: preSharedKey -> Tot (b:bytes{length b >= 2})
-let preSharedKeyBytes = function
-  | ClientPreSharedKey cpsk -> clientPreSharedKeyBytes cpsk
-  | ServerPreSharedKey spsk -> serverPreSharedKeyBytes spsk
-
-(** Parsing function for PreSharedKey *)
-val parsePreSharedKey: pinverse_t preSharedKeyBytes
-let parsePreSharedKey b =
-  match vlparse 2 b with
-  | Correct b' ->
-    begin
-      match vlparse 2 b with
-      | Correct b'' -> // Client case
-	begin
-	if length b >= 2 && length b < 65538 then
-	  begin
-	  match parseClientPreSharedKey b with
-	  | Correct psks -> Correct (ClientPreSharedKey psks)
-	  | Error z -> Error z
-	  end
-	else Error(AD_decode_error, perror __SOURCE_FILE__ __LINE__ "Failed to parse  psk")
-	end
-      | Error _ -> // Server case
-	begin
-	match parseServerPreSharedKey b with
-	| Correct psk -> Correct (ServerPreSharedKey psk)
-	| Error z -> Error z
-	end
-    end
-  | Error z -> Error(AD_decode_error, perror __SOURCE_FILE__ __LINE__ "Failed to parse pre shared key")
