src/tls/TLSFormats.fst
@@ -1,0 +1,1555 @@
+module TLSFormats
+
+(**
+This file implements seraliazation and parsing functions
+for the different values negotiated during the TLS
+handshake. For instance protocol version, key exchange mechanism,
+hash algorithm etc.
+
+@summary Module for serialization and parsing
+*)
+
+#set-options "--max_fuel 0 --initial_fuel 0 --max_ifuel 1 --initial_ifuel 1"
+
+open FStar.SeqProperties
+open Platform.Bytes
+open Platform.Error
+open TLSError
+open CoreCrypto
+open TLSConstants
+
+module HH = FStar.HyperHeap
+module HS = FStar.HyperStack
+
+
+(* This is the old version of the inverse predicate. According to CF,
+   verification was harder with this style, so we moved to the new style with
+   pinverse_t + lemmas. The type abbrevations lemma_inverse_* minimize the
+   syntactic overhead.
+
+  logic type pinverse (#a:Type) (#b:Type) (r:b -> b -> Type) (=f:a -> Tot b) =
+    y:b -> Tot (xopt:result a{(forall (x:a). r (f x) y <==> (xopt = Correct x))})
+*)
+
+type pinverse_t (#a:Type) (#b:Type) ($f:(a -> Tot b)) = b -> Tot (result a)
+
+unfold type lemma_inverse_g_f (#a:Type) (#b:Type) ($f:a -> Tot b) ($g:b -> Tot (result a)) (x:a) =
+  g (f x) == Correct x
+
+unfold type lemma_pinverse_f_g (#a:Type) (#b:Type) (r:b -> b -> Type) ($f:a -> Tot b) ($g:b -> Tot (result a)) (y:b) =
+  is_Correct (g y) ==> r (f (Correct._0 (g y))) y
+
+
+(** Serializing function for signature algorithms *)
+val sigAlgBytes: sigAlg -> Tot (lbytes 1)
+let sigAlgBytes sa =
+  match sa with
+  | CoreCrypto.RSASIG -> abyte 1z
+  | CoreCrypto.DSA    -> abyte 2z
+  | CoreCrypto.ECDSA  -> abyte 3z
+  | CoreCrypto.RSAPSS -> abyte 0z // TODO fix me!
+
+(** Parsing function associated to sigAlgBytes *)
+val parseSigAlg: pinverse_t sigAlgBytes
+let parseSigAlg b =
+  match cbyte b with
+  | 1z -> Correct CoreCrypto.RSASIG
+  | 2z -> Correct CoreCrypto.DSA
+  | 3z -> Correct CoreCrypto.ECDSA
+  | 0z -> Correct CoreCrypto.RSAPSS
+  | _ -> Error (AD_decode_error, perror __SOURCE_FILE__ __LINE__ "")
+
+val inverse_sigAlg: x:_ -> Lemma
+  (requires (True))
+  (ensures lemma_inverse_g_f sigAlgBytes parseSigAlg x)
+  [SMTPat (parseSigAlg (sigAlgBytes x))]
+let inverse_sigAlg x = ()
+
+val pinverse_sigAlg: x:_ -> Lemma
+  (requires (True))
+  (ensures (lemma_pinverse_f_g Seq.equal sigAlgBytes parseSigAlg x))
+  [SMTPat (sigAlgBytes (Correct._0 (parseSigAlg x)))]
+let pinverse_sigAlg x = ()
+
+
+#set-options "--max_fuel 0 --initial_fuel 0 --max_ifuel 2 --initial_ifuel 2"
+
+(** Serializing of the Hash algorithm *)
+val hashAlgBytes: hashAlg' -> Tot (lbytes 1)
+let hashAlgBytes ha =
+  match ha with
+  | Hash MD5     -> abyte 1z
+  | Hash SHA1    -> abyte 2z
+  | Hash SHA224  -> abyte 3z
+  | Hash SHA256  -> abyte 4z
+  | Hash SHA384  -> abyte 5z
+  | Hash SHA512  -> abyte 6z
+  | NULL -> abyte 7z // FIXME!!
+
+(** Parsing of the Hash algorithm *)
+val parseHashAlg: pinverse_t hashAlgBytes
+let parseHashAlg b =
+  match cbyte b with
+  | 1z -> Correct (Hash MD5)
+  | 2z -> Correct (Hash SHA1)
+  | 3z -> Correct (Hash SHA224)
+  | 4z -> Correct (Hash SHA256)
+  | 5z -> Correct (Hash SHA384)
+  | 6z -> Correct (Hash SHA512)
+  | 7z -> admit();  //TODO: FIXME!!!!
+         Correct (NULL)
+  | _ -> Error (AD_decode_error, perror __SOURCE_FILE__ __LINE__ "")
+
+val inverse_hashAlg: x:_ -> Lemma
+  (requires (True))
+  (ensures lemma_inverse_g_f hashAlgBytes parseHashAlg x)
+  [SMTPat (parseHashAlg (hashAlgBytes x))]
+let inverse_hashAlg x = ()
+
+val pinverse_hashAlg: x:_ -> Lemma
+  (requires (True))
+  (ensures (lemma_pinverse_f_g Seq.equal hashAlgBytes parseHashAlg x))
+  [SMTPat (hashAlgBytes (Correct._0 (parseHashAlg x)))]
+let pinverse_hashAlg x = ()
+
+(** Serializing function for compression algorithms *)
+val compressionBytes: compression -> Tot (lbytes 1)
+let compressionBytes comp =
+  match comp with
+  | NullCompression      -> abyte 0z
+  | UnknownCompression b -> abyte b
+
+// Not pinverse_t compressionBytes, because it never fails
+
+(** Parsing function for compression algorithm *)
+val parseCompression: b:lbytes 1
+  -> Tot (cm:compression{Seq.equal (compressionBytes cm) b})
+let parseCompression b =
+  match cbyte b with
+  | 0z -> NullCompression
+  | b  -> UnknownCompression b
+
+// We ignore compression methods we don't understand. This is a departure
+// from usual parsing, where we fail on unknown values, but that's how TLS
+// handles compression method lists.
+
+(** Parsing function for compression algorithm lists *)
+val parseCompressions: b:bytes -> Tot (list compression) (decreases (length b))
+let rec parseCompressions b =
+  if length b > 0
+  then
+    let cmB,b = split b 1 in
+    let cm = parseCompression cmB in
+    cm::(parseCompressions b)
+  else []
+
+
+#set-options "--max_fuel 1 --initial_fuel 1 --max_ifuel 1 --initial_ifuel 1"
+
+(** Serializing function for lists of compression algorithms *)
+val compressionMethodsBytes: cms:list compression
+  -> Tot (lbytes (List.Tot.length cms))
+let rec compressionMethodsBytes cms =
+  match cms with
+  | c::cs -> compressionBytes c @| compressionMethodsBytes cs
+  | []   -> empty_bytes
+
+
+#set-options "--max_fuel 0 --initial_fuel 0 --max_ifuel 1 --initial_ifuel 1"
+
+(** Serializing function for the protocol version *)
+val versionBytes: protocolVersion -> Tot (lbytes 2)
+let versionBytes pv =
+  match pv with
+  | SSL_3p0 -> abyte2 ( 3z, 0z)
+  | TLS_1p0 -> abyte2 ( 3z, 1z)
+  | TLS_1p1 -> abyte2 ( 3z, 2z )
+  | TLS_1p2 -> abyte2 ( 3z, 3z )
+  | TLS_1p3 -> abyte2 ( 3z, 4z )
+
+(** Parsing function for the protocol version *)
+val parseVersion: pinverse_t versionBytes
+let parseVersion v =
+  match cbyte2 v with
+  | ( 3z, 0z ) -> Correct SSL_3p0
+  | ( 3z, 1z ) -> Correct TLS_1p0
+  | ( 3z, 2z ) -> Correct TLS_1p1
+  | ( 3z, 3z ) -> Correct TLS_1p2
+  | ( 3z, 4z ) -> Correct TLS_1p3
+  | _ -> Error(AD_decode_error, perror __SOURCE_FILE__ __LINE__ "Parsed an unknown version")
+
+val inverse_version: x:_ -> Lemma
+  (requires (True))
+  (ensures lemma_inverse_g_f versionBytes parseVersion x)
+  [SMTPat (parseVersion (versionBytes x))]
+let inverse_version x = ()
+
+val pinverse_version: x:_ -> Lemma
+  (requires (True))
+  (ensures (lemma_pinverse_f_g Seq.equal versionBytes parseVersion x))
+  [SMTPat (versionBytes (Correct._0 (parseVersion x)))]
+let pinverse_version x = ()
+
+(* JK: injectivity proof requires extra specification for the UnknownCipherSuite objects as they
+   have to be distinct from the 'correct' ones *)
+val cipherSuiteBytesOpt: cipherSuite -> Tot (option (lbytes 2))
+let cipherSuiteBytesOpt cs =
+  let abyte2 b: option (lbytes 2) = Some (abyte2 b) in
+    match cs with
+    | UnknownCipherSuite b1 b2 -> abyte2 (b1,b2)
+    | NullCipherSuite                                              -> abyte2 ( 0x00z, 0x00z )
+
+    | CipherSuite Kex_RSA None (MACOnly MD5)                       -> abyte2 ( 0x00z, 0x01z )
+    | CipherSuite Kex_RSA None (MACOnly SHA1)                      -> abyte2 ( 0x00z, 0x02z )
+    | CipherSuite Kex_RSA None (MACOnly SHA256)                    -> abyte2 ( 0x00z, 0x3Bz )
+    | CipherSuite Kex_RSA None(MtE (Stream RC4_128) MD5)           -> abyte2 ( 0x00z, 0x04z )
+    | CipherSuite Kex_RSA None(MtE (Stream RC4_128) SHA1)          -> abyte2 ( 0x00z, 0x05z )
+
+    | CipherSuite Kex_RSA None(MtE (Block TDES_EDE_CBC) SHA1)      -> abyte2 ( 0x00z, 0x0Az )
+    | CipherSuite Kex_RSA None(MtE (Block AES_128_CBC) SHA1)       -> abyte2 ( 0x00z, 0x2Fz )
+    | CipherSuite Kex_RSA None(MtE (Block AES_256_CBC) SHA1)       -> abyte2 ( 0x00z, 0x35z )
+    | CipherSuite Kex_RSA None(MtE (Block AES_128_CBC) SHA256)     -> abyte2 ( 0x00z, 0x3Cz )
+    | CipherSuite Kex_RSA None(MtE (Block AES_256_CBC) SHA256)     -> abyte2 ( 0x00z, 0x3Dz )
+
+    (**************************************************************************)
+    | CipherSuite Kex_DH (Some DSA)     (MtE (Block TDES_EDE_CBC) SHA1)   -> abyte2 ( 0x00z, 0x0Dz )
+    | CipherSuite Kex_DH (Some RSASIG)  (MtE (Block TDES_EDE_CBC) SHA1)   -> abyte2 ( 0x00z, 0x10z )
+    | CipherSuite Kex_DHE (Some DSA)    (MtE (Block TDES_EDE_CBC) SHA1)   -> abyte2 ( 0x00z, 0x13z )
+    | CipherSuite Kex_DHE (Some RSASIG) (MtE (Block TDES_EDE_CBC) SHA1)   -> abyte2 ( 0x00z, 0x16z )
+
+    | CipherSuite Kex_DH (Some DSA)     (MtE (Block AES_128_CBC) SHA1)    -> abyte2 ( 0x00z, 0x30z )
+    | CipherSuite Kex_DH (Some RSASIG)  (MtE (Block AES_128_CBC) SHA1)    -> abyte2 ( 0x00z, 0x31z )
+    | CipherSuite Kex_DHE (Some DSA)    (MtE (Block AES_128_CBC) SHA1)    -> abyte2 ( 0x00z, 0x32z )
+    | CipherSuite Kex_DHE (Some RSASIG) (MtE (Block AES_128_CBC) SHA1)    -> abyte2 ( 0x00z, 0x33z )
+
+    | CipherSuite Kex_DH (Some DSA)     (MtE (Block AES_256_CBC) SHA1)    -> abyte2 ( 0x00z, 0x36z )
+    | CipherSuite Kex_DH (Some RSASIG)  (MtE (Block AES_256_CBC) SHA1)    -> abyte2 ( 0x00z, 0x37z )
+    | CipherSuite Kex_DHE (Some DSA)    (MtE (Block AES_256_CBC) SHA1)    -> abyte2 ( 0x00z, 0x38z )
+    | CipherSuite Kex_DHE (Some RSASIG) (MtE (Block AES_256_CBC) SHA1)    -> abyte2 ( 0x00z, 0x39z )
+
+    | CipherSuite Kex_DH (Some DSA)     (MtE (Block AES_128_CBC) SHA256)  -> abyte2 ( 0x00z, 0x3Ez )
+    | CipherSuite Kex_DH (Some RSASIG)  (MtE (Block AES_128_CBC) SHA256)  -> abyte2 ( 0x00z, 0x3Fz )
+    | CipherSuite Kex_DHE (Some DSA)    (MtE (Block AES_128_CBC) SHA256)  -> abyte2 ( 0x00z, 0x40z )
+    | CipherSuite Kex_DHE (Some RSASIG) (MtE (Block AES_128_CBC) SHA256)  -> abyte2 ( 0x00z, 0x67z )
+
+    | CipherSuite Kex_DH (Some DSA)     (MtE (Block AES_256_CBC) SHA256)  -> abyte2 ( 0x00z, 0x68z )
+    | CipherSuite Kex_DH (Some RSASIG)  (MtE (Block AES_256_CBC) SHA256)  -> abyte2 ( 0x00z, 0x69z )
+    | CipherSuite Kex_DHE (Some DSA)    (MtE (Block AES_256_CBC) SHA256)  -> abyte2 ( 0x00z, 0x6Az )
+    | CipherSuite Kex_DHE (Some RSASIG) (MtE (Block AES_256_CBC) SHA256)  -> abyte2 ( 0x00z, 0x6Bz )
+
+    (**************************************************************************)
+    | CipherSuite Kex_ECDHE (Some RSASIG) (MtE (Stream RC4_128) SHA1)       -> abyte2 ( 0xc0z, 0x11z )
+    | CipherSuite Kex_ECDHE (Some RSASIG) (MtE (Block TDES_EDE_CBC) SHA1)   -> abyte2 ( 0xc0z, 0x12z )
+    | CipherSuite Kex_ECDHE (Some RSASIG) (MtE (Block AES_128_CBC) SHA1)    -> abyte2 ( 0xc0z, 0x13z )
+    | CipherSuite Kex_ECDHE (Some RSASIG) (MtE (Block AES_256_CBC) SHA1)    -> abyte2 ( 0xc0z, 0x14z )
+    | CipherSuite Kex_ECDHE (Some RSASIG) (MtE (Block AES_128_CBC) SHA256)  -> abyte2 ( 0xc0z, 0x27z )
+    | CipherSuite Kex_ECDHE (Some RSASIG) (MtE (Block AES_256_CBC) SHA384)  -> abyte2 ( 0xc0z, 0x28z )
+
+    | CipherSuite Kex_ECDHE (Some RSASIG) (AEAD AES_128_GCM SHA256) -> abyte2 ( 0xc0z, 0x2fz )
+    | CipherSuite Kex_ECDHE (Some ECDSA)  (AEAD AES_128_GCM SHA256) -> abyte2 ( 0xc0z, 0x2bz )
+    | CipherSuite Kex_ECDHE (Some RSASIG) (AEAD AES_256_GCM SHA384) -> abyte2 ( 0xc0z, 0x30z )
+    | CipherSuite Kex_ECDHE (Some ECDSA) (AEAD AES_256_GCM SHA384) -> abyte2 ( 0xc0z, 0x2cz )
+
+    (**************************************************************************)
+    | CipherSuite Kex_PSK_DHE None (AEAD AES_128_GCM SHA256) -> abyte2 ( 0x00z, 0xaaz )
+    | CipherSuite Kex_PSK_DHE None (AEAD AES_256_GCM SHA384) -> abyte2 ( 0x00z, 0xabz )
+    | CipherSuite Kex_PSK_ECDHE None (AEAD AES_128_GCM SHA256) -> abyte2 ( 0xd0z, 0x01z )
+    | CipherSuite Kex_PSK_ECDHE None (AEAD AES_256_GCM SHA384) -> abyte2 ( 0xd0z, 0x02z )
+
+    (**************************************************************************)
+    | CipherSuite Kex_DHE None   (MtE (Stream RC4_128) MD5)         -> abyte2 ( 0x00z, 0x18z )
+    | CipherSuite Kex_DHE None   (MtE (Block TDES_EDE_CBC) SHA1)    -> abyte2 ( 0x00z, 0x1Bz )
+    | CipherSuite Kex_DHE None   (MtE (Block AES_128_CBC) SHA1)     -> abyte2 ( 0x00z, 0x34z )
+    | CipherSuite Kex_DHE None   (MtE (Block AES_256_CBC) SHA1)     -> abyte2 ( 0x00z, 0x3Az )
+    | CipherSuite Kex_DHE None   (MtE (Block AES_128_CBC) SHA256)   -> abyte2 ( 0x00z, 0x6Cz )
+    | CipherSuite Kex_DHE None   (MtE (Block AES_256_CBC) SHA256)   -> abyte2 ( 0x00z, 0x6Dz )
+
+    (**************************************************************************)
+    | CipherSuite Kex_RSA None     (AEAD AES_128_GCM SHA256) -> abyte2( 0x00z, 0x9Cz )
+    | CipherSuite Kex_RSA None     (AEAD AES_256_GCM SHA384) -> abyte2( 0x00z, 0x9Dz )
+
+    | CipherSuite Kex_DHE (Some RSASIG) (AEAD AES_128_GCM SHA256) -> abyte2( 0x00z, 0x9Ez )
+    | CipherSuite Kex_DHE (Some RSASIG) (AEAD AES_256_GCM SHA384) -> abyte2( 0x00z, 0x9Fz )
+    | CipherSuite Kex_DH (Some RSASIG)  (AEAD AES_128_GCM SHA256) -> abyte2( 0x00z, 0xA0z )
+    | CipherSuite Kex_DH (Some RSASIG)  (AEAD AES_256_GCM SHA384) -> abyte2( 0x00z, 0xA1z )
+
+    | CipherSuite Kex_DHE (Some DSA) (AEAD AES_128_GCM SHA256) -> abyte2( 0x00z, 0xA2z )
+    | CipherSuite Kex_DHE (Some DSA) (AEAD AES_256_GCM SHA384) -> abyte2( 0x00z, 0xA3z )
+    | CipherSuite Kex_DH (Some DSA)  (AEAD AES_128_GCM SHA256) -> abyte2( 0x00z, 0xA4z )
+    | CipherSuite Kex_DH (Some DSA)  (AEAD AES_256_GCM SHA384) -> abyte2( 0x00z, 0xA5z )
+
+    | CipherSuite Kex_DHE None (AEAD AES_128_GCM SHA256) -> abyte2( 0x00z, 0xA6z )
+    | CipherSuite Kex_DHE None (AEAD AES_256_GCM SHA384) -> abyte2( 0x00z, 0xA7z )
+
+    | SCSV (TLS_EMPTY_RENEGOTIATION_INFO_SCSV)         -> abyte2 ( 0x00z, 0xFFz )
+    | _ -> None
+
+(** Determine if a ciphersuite is valid *)
+let validCipherSuite (c:cipherSuite) = is_Some (cipherSuiteBytesOpt c)
+let valid_cipher_suite = c:cipherSuite{validCipherSuite c}
+
+(** List of valid ciphersuite *)
+let valid_cipher_suites = list valid_cipher_suite
+
+(** Serializing function for a valid ciphersuite *)
+val cipherSuiteBytes: valid_cipher_suite -> Tot (lbytes 2)
+let cipherSuiteBytes c = Some.v (cipherSuiteBytesOpt c)
+
+
+(** Auxillary parsing function for ciphersuites *)
+val parseCipherSuiteAux : lbytes 2 -> Tot (result (c:cipherSuite{validCipherSuite c}))
+let parseCipherSuiteAux b =
+  match cbyte2 b with
+  | ( 0x00z, 0x00z ) -> Correct(NullCipherSuite)
+
+  | ( 0x00z, 0x01z ) -> Correct(CipherSuite Kex_RSA None (MACOnly MD5))
+  | ( 0x00z, 0x02z ) -> Correct(CipherSuite Kex_RSA None (MACOnly SHA1))
+  | ( 0x00z, 0x3Bz ) -> Correct(CipherSuite Kex_RSA None (MACOnly SHA256))
+  | ( 0x00z, 0x04z ) -> Correct(CipherSuite Kex_RSA None (MtE (Stream RC4_128) MD5))
+  | ( 0x00z, 0x05z ) -> Correct(CipherSuite Kex_RSA None (MtE (Stream RC4_128) SHA1))
+
+  | ( 0x00z, 0x0Az ) -> Correct(CipherSuite Kex_RSA None (MtE (Block TDES_EDE_CBC) SHA1))
+  | ( 0x00z, 0x2Fz ) -> Correct(CipherSuite Kex_RSA None (MtE (Block AES_128_CBC) SHA1))
+  | ( 0x00z, 0x35z ) -> Correct(CipherSuite Kex_RSA None (MtE (Block AES_256_CBC) SHA1))
+  | ( 0x00z, 0x3Cz ) -> Correct(CipherSuite Kex_RSA None (MtE (Block AES_128_CBC) SHA256))
+  | ( 0x00z, 0x3Dz ) -> Correct(CipherSuite Kex_RSA None (MtE (Block AES_256_CBC) SHA256))
+
+  (**************************************************************************)
+  | ( 0x00z, 0x0Dz ) -> Correct(CipherSuite Kex_DH (Some DSA) (MtE (Block TDES_EDE_CBC) SHA1))
+  | ( 0x00z, 0x10z ) -> Correct(CipherSuite Kex_DH (Some RSASIG) (MtE (Block TDES_EDE_CBC) SHA1))
+  | ( 0x00z, 0x13z ) -> Correct(CipherSuite Kex_DHE (Some DSA) (MtE (Block TDES_EDE_CBC) SHA1))
+  | ( 0x00z, 0x16z ) -> Correct(CipherSuite Kex_DHE (Some RSASIG) (MtE (Block TDES_EDE_CBC) SHA1))
+
+  | ( 0x00z, 0x30z ) -> Correct(CipherSuite Kex_DH (Some DSA) (MtE (Block AES_128_CBC) SHA1))
+  | ( 0x00z, 0x31z ) -> Correct(CipherSuite Kex_DH (Some RSASIG) (MtE (Block AES_128_CBC) SHA1))
+  | ( 0x00z, 0x32z ) -> Correct(CipherSuite Kex_DHE (Some DSA) (MtE (Block AES_128_CBC) SHA1))
+  | ( 0x00z, 0x33z ) -> Correct(CipherSuite Kex_DHE (Some RSASIG) (MtE (Block AES_128_CBC) SHA1))
+
+  | ( 0x00z, 0x36z ) -> Correct(CipherSuite Kex_DH (Some DSA) (MtE (Block AES_256_CBC) SHA1))
+  | ( 0x00z, 0x37z ) -> Correct(CipherSuite Kex_DH (Some RSASIG) (MtE (Block AES_256_CBC) SHA1))
+  | ( 0x00z, 0x38z ) -> Correct(CipherSuite Kex_DHE (Some DSA) (MtE (Block AES_256_CBC) SHA1))
+  | ( 0x00z, 0x39z ) -> Correct(CipherSuite Kex_DHE (Some RSASIG) (MtE (Block AES_256_CBC) SHA1))
+
+  | ( 0x00z, 0x3Ez ) -> Correct(CipherSuite Kex_DH (Some DSA) (MtE (Block AES_128_CBC) SHA256))
+  | ( 0x00z, 0x3Fz ) -> Correct(CipherSuite Kex_DH (Some RSASIG) (MtE (Block AES_128_CBC) SHA256))
+  | ( 0x00z, 0x40z ) -> Correct(CipherSuite Kex_DHE (Some DSA) (MtE (Block AES_128_CBC) SHA256))
+  | ( 0x00z, 0x67z ) -> Correct(CipherSuite Kex_DHE (Some RSASIG) (MtE (Block AES_128_CBC) SHA256))
+
+  | ( 0x00z, 0x68z ) -> Correct(CipherSuite Kex_DH (Some DSA) (MtE (Block AES_256_CBC) SHA256))
+  | ( 0x00z, 0x69z ) -> Correct(CipherSuite Kex_DH (Some RSASIG) (MtE (Block AES_256_CBC) SHA256))
+  | ( 0x00z, 0x6Az ) -> Correct(CipherSuite Kex_DHE (Some DSA) (MtE (Block AES_256_CBC) SHA256))
+  | ( 0x00z, 0x6Bz ) -> Correct(CipherSuite Kex_DHE (Some RSASIG) (MtE (Block AES_256_CBC) SHA256))
+
+  (**************************************************************************)
+  | ( 0xc0z, 0x11z ) -> Correct(CipherSuite Kex_ECDHE (Some RSASIG) (MtE (Stream RC4_128) SHA1))
+  | ( 0xc0z, 0x12z ) -> Correct(CipherSuite Kex_ECDHE (Some RSASIG) (MtE (Block TDES_EDE_CBC) SHA1))
+  | ( 0xc0z, 0x13z ) -> Correct(CipherSuite Kex_ECDHE (Some RSASIG) (MtE (Block AES_128_CBC) SHA1))
+  | ( 0xc0z, 0x14z ) -> Correct(CipherSuite Kex_ECDHE (Some RSASIG) (MtE (Block AES_256_CBC) SHA1))
+  | ( 0xc0z, 0x27z ) -> Correct(CipherSuite Kex_ECDHE (Some RSASIG) (MtE (Block AES_128_CBC) SHA256))
+  | ( 0xc0z, 0x28z ) -> Correct(CipherSuite Kex_ECDHE (Some RSASIG) (MtE (Block AES_256_CBC) SHA384))
+
+  (**************************************************************************)
+  | ( 0xc0z, 0x2bz ) -> Correct(CipherSuite Kex_ECDHE (Some ECDSA) (AEAD AES_128_GCM SHA256))
+  | ( 0xc0z, 0x2fz ) -> Correct(CipherSuite Kex_ECDHE (Some RSASIG) (AEAD AES_128_GCM SHA256))
+  | ( 0xc0z, 0x2cz ) -> Correct(CipherSuite Kex_ECDHE (Some ECDSA) (AEAD AES_256_GCM SHA384))
+  | ( 0xc0z, 0x30z ) -> Correct(CipherSuite Kex_ECDHE (Some RSASIG) (AEAD AES_256_GCM SHA384))
+
+  (**************************************************************************)
+  | ( 0xd0z, 0x01z ) -> Correct(CipherSuite Kex_PSK_ECDHE None (AEAD AES_128_GCM SHA256))
+  | ( 0xd0z, 0x02z ) -> Correct(CipherSuite Kex_PSK_ECDHE None (AEAD AES_256_GCM SHA384))
+
+  (**************************************************************************)
+  | ( 0x00z, 0x18z ) -> Correct(CipherSuite Kex_DHE None (MtE (Stream RC4_128) MD5))
+  | ( 0x00z, 0x1Bz ) -> Correct(CipherSuite Kex_DHE None (MtE (Block TDES_EDE_CBC) SHA1))
+  | ( 0x00z, 0x34z ) -> Correct(CipherSuite Kex_DHE None (MtE (Block AES_128_CBC) SHA1))
+  | ( 0x00z, 0x3Az ) -> Correct(CipherSuite Kex_DHE None (MtE (Block AES_256_CBC) SHA1))
+  | ( 0x00z, 0x6Cz ) -> Correct(CipherSuite Kex_DHE None (MtE (Block AES_128_CBC) SHA256))
+  | ( 0x00z, 0x6Dz ) -> Correct(CipherSuite Kex_DHE None (MtE (Block AES_256_CBC) SHA256))
+
+  (**************************************************************************)
+  | ( 0x00z, 0x9Cz ) -> Correct(CipherSuite Kex_RSA None (AEAD AES_128_GCM SHA256))
+  | ( 0x00z, 0x9Dz ) -> Correct(CipherSuite Kex_RSA None (AEAD AES_256_GCM SHA384))
+
+  | ( 0x00z, 0x9Ez ) -> Correct(CipherSuite Kex_DHE (Some RSASIG) (AEAD AES_128_GCM SHA256))
+  | ( 0x00z, 0x9Fz ) -> Correct(CipherSuite Kex_DHE (Some RSASIG) (AEAD AES_256_GCM SHA384))
+  | ( 0x00z, 0xA0z ) -> Correct(CipherSuite Kex_DH (Some RSASIG)  (AEAD AES_128_GCM SHA256))
+  | ( 0x00z, 0xA1z ) -> Correct(CipherSuite Kex_DH (Some RSASIG)  (AEAD AES_256_GCM SHA384))
+
+  | ( 0x00z, 0xA2z ) -> Correct(CipherSuite Kex_DHE (Some DSA) (AEAD AES_128_GCM SHA256))
+  | ( 0x00z, 0xA3z ) -> Correct(CipherSuite Kex_DHE (Some DSA) (AEAD AES_256_GCM SHA384))
+  | ( 0x00z, 0xA4z ) -> Correct(CipherSuite Kex_DH (Some DSA)  (AEAD AES_128_GCM SHA256))
+  | ( 0x00z, 0xA5z ) -> Correct(CipherSuite Kex_DH (Some DSA)  (AEAD AES_256_GCM SHA384))
+
+  | ( 0x00z, 0xA6z ) -> Correct(CipherSuite Kex_DHE None (AEAD AES_128_GCM SHA256))
+  | ( 0x00z, 0xA7z ) -> Correct(CipherSuite Kex_DHE None (AEAD AES_256_GCM SHA384))
+
+  (**************************************************************************)
+  | ( 0x00z, 0xaaz ) -> Correct(CipherSuite Kex_PSK_DHE None (AEAD AES_128_GCM SHA256))
+  | ( 0x00z, 0xabz ) -> Correct(CipherSuite Kex_PSK_DHE None (AEAD AES_256_GCM SHA384))
+
+  (**************************************************************************)
+  | ( 0x00z, 0xFFz ) -> Correct(SCSV (TLS_EMPTY_RENEGOTIATION_INFO_SCSV))
+  | (b1, b2) -> Correct(UnknownCipherSuite b1 b2)
+// Was:  | _ -> Error(AD_decode_error, perror __SOURCE_FILE__ __LINE__ "Parsed unknown cipher")
+
+(** Parsing function for ciphersuites *)
+val parseCipherSuite: pinverse_t cipherSuiteBytes
+let parseCipherSuite b =
+  match parseCipherSuiteAux b with
+  | Correct c -> Correct c
+  | Error z -> Error z
+
+
+//#reset-options "--z3rlimit 60 --max_ifuel 6 --initial_ifuel 6 --max_fuel 1 --initial_fuel 1"
+
+(** Lemma for ciphersuite serializing/parsing inversions *)
+val inverse_cipherSuite: x:cipherSuite -> Lemma
+  (requires (~ (is_UnknownCipherSuite x)))
+  // parse (bytes (Unknown 0 0)) = NullCiphersuite
+  // must exclude this case...
+  (ensures (let y = cipherSuiteBytesOpt x in
+	(is_Some y ==> parseCipherSuiteAux (Some.v y) = Correct x)))
+  [SMTPat (parseCipherSuiteAux (Some.v (cipherSuiteBytesOpt x)))]
+let inverse_cipherSuite x = ()
+
+(** Lemma for ciphersuite serializing/parsing inversions *)
+val pinverse_cipherSuite : x:lbytes 2 -> Lemma
+  (requires (True))
+  (ensures (let y = parseCipherSuiteAux x in
+	    (is_Correct y ==>
+              (if is_UnknownCipherSuite (Correct._0 y) then true
+              else is_Some (cipherSuiteBytesOpt (Correct._0 y))
+               /\ Seq.equal x (Some.v (cipherSuiteBytesOpt (Correct._0 y)))))))
+  [SMTPat (cipherSuiteBytesOpt (Correct._0 (parseCipherSuiteAux x)))]
+let pinverse_cipherSuite x = ()
+
+
+#reset-options
+#set-options "--max_ifuel 1 --initial_ifuel 1 --max_fuel 1 --initial_fuel 1"
+
+(** Serializing function for a list of ciphersuite *)
+val cipherSuitesBytes: css:list (c:cipherSuite{validCipherSuite c}) -> Tot (lbytes (op_Multiply 2 (List.Tot.length css)))
+let rec cipherSuitesBytes css =
+  match css with
+  | [] -> empty_bytes
+  | cs::css -> (cipherSuiteBytes cs) @| (cipherSuitesBytes css)
+
+// Called by the server handshake;
+// ciphersuites that we do not understand are parsed, but ignored
+
+(** Parsing function for a list of ciphersuites *)
+val parseCipherSuites: b:bytes -> Tot (result (list (c:cipherSuite{validCipherSuite c}))) (decreases (length b))
+let rec parseCipherSuites b =
+  if length b > 1 then
+    let (b0,b1) = split b 2 in
+    match parseCipherSuites b1 with
+      | Correct(css) ->
+	(match parseCipherSuite b0 with
+	 | Error z ->	Correct css
+	 | Correct cs -> Correct (cs::css))
+      | Error z -> Error z
+  else
+  if length b = 0 then Correct []
+  else Error(AD_decode_error, perror __SOURCE_FILE__ __LINE__ "Odd cs bytes number")
+
+
+#reset-options
+#set-options "--max_ifuel 2 --initial_ifuel 2 --max_fuel 2 --initial_fuel 2"
+
+(** Lemma for ciphersuite lists serializing/parsing inversions *)
+val inverse_cipherSuites: x:list (c:cipherSuite{validCipherSuite c}) -> Lemma
+  (requires (true))
+  (ensures (parseCipherSuites (cipherSuitesBytes x) = Correct x))
+  [SMTPat (parseCipherSuites (cipherSuitesBytes x))]
+let rec inverse_cipherSuites x =
+  match x with
+  | [] -> ()
+  | cs::css ->
+     assume (~ (is_UnknownCipherSuite cs)); // TODO enforce it
+     let b = (cipherSuiteBytes cs) @| (cipherSuitesBytes css) in
+     let (b0,b1) = split b 2 in
+     lemma_append_inj b0 b1 (cipherSuiteBytes cs) (cipherSuitesBytes css);
+     inverse_cipherSuite cs;
+     inverse_cipherSuites css
+
+// REMARK: cipherSuitesBytes is not a partial inverse of parseCipherSuites,
+// because parseCipherSuites drops unknown ciphersuites.
+// Alternatively, we could add an UNKNOWN of (lbyte 2) constructor in cipherSuite
+// to make this hold.
+//
+// TODO: We added such constructor, so this is the case now. Prove it.
+
+
+// Note:
+// Migrated contentType to Content.fst (this is internal to TLS)
+
+(** Transforms a sequence of natural numbers into bytes *)
+val bytes_of_seq: n:nat{ repr_bytes n <= 8 } -> Tot bytes
+let bytes_of_seq sn = bytes_of_int 8 sn
+
+(** Transforms bytes into a sequence of natural numbers *)
+val seq_of_bytes: b:bytes{ length b <= 8 } -> Tot nat
+let seq_of_bytes b = int_of_bytes b
+
+(** Transform and concatenate a natural number to bytes *)
+val vlbytes: lSize:nat -> b:bytes{repr_bytes (length b) <= lSize} -> Tot (r:bytes{length r = lSize + length b})
+let vlbytes lSize b = bytes_of_int lSize (length b) @| b
+
+(** Lemmas associated to bytes manipulations *)
+val lemma_vlbytes_len : i:nat -> b:bytes{repr_bytes (length b) <= i}
+  -> Lemma (ensures (length (vlbytes i b) = i + length b))
+let lemma_vlbytes_len i b = ()
+
+val lemma_vlbytes_inj : i:nat
+  -> b:bytes{repr_bytes (length b) <= i}
+  -> b':bytes{repr_bytes (length b') <= i}
+  -> Lemma (requires (Seq.equal (vlbytes i b) (vlbytes i b')))
+          (ensures (b == b'))
+let lemma_vlbytes_inj i b b' =
+  let l = bytes_of_int i (length b) in
+  SeqProperties.lemma_append_inj l b l b'
+
+val vlbytes_length_lemma: n:nat -> a:bytes{repr_bytes (length a) <= n} -> b:bytes{repr_bytes (length b) <= n} -> 
+  Lemma (requires (Seq.equal (Seq.slice (vlbytes n a) 0 n) (Seq.slice (vlbytes n b) 0 n)))
+        (ensures (length a = length b))
+let vlbytes_length_lemma n a b = 
+  let lena = Seq.slice (vlbytes n a) 0 n in
+  let lenb = Seq.slice (vlbytes n b) 0 n in
+  assert(Seq.equal lena (bytes_of_int n (length a)));
+  assert(Seq.equal lenb (bytes_of_int n (length b)));
+  int_of_bytes_of_int n (length a); int_of_bytes_of_int n (length b)
+
+
+#set-options "--max_ifuel 1 --initial_ifuel 1 --max_fuel 0 --initial_fuel 0"   //need to reason about length
+
+
+val vlsplit: lSize:nat{lSize <= 4}
+  -> vlb:bytes{lSize <= length vlb}
+  -> Tot (result (b:(bytes * bytes){
+                    repr_bytes (length (fst b)) <= lSize
+                  /\ Seq.equal vlb (vlbytes lSize (fst b) @| (snd b))}))
+let vlsplit lSize vlb =
+  let (vl,b) = Platform.Bytes.split vlb lSize in
+  let l = int_of_bytes vl in
+  if l <= length b
+  then Correct(Platform.Bytes.split b l)
+  else Error(AD_decode_error, perror __SOURCE_FILE__ __LINE__ "")
+
+
+val vlparse: lSize:nat{lSize <= 4} -> vlb:bytes{lSize <= length vlb}
+  -> Tot (result (b:bytes{repr_bytes (length b) <= lSize /\ Seq.equal vlb (vlbytes lSize b)}))
+let vlparse lSize vlb =
+  let vl,b = split vlb lSize in
+  if int_of_bytes vl = length b
+  then Correct b
+  else Error(AD_decode_error, perror __SOURCE_FILE__ __LINE__ "")
+
+
+val vlparse_vlbytes: lSize:nat{lSize <= 4} -> vlb:bytes{repr_bytes (length vlb) <= lSize} -> Lemma 
+  (requires (True))
+  (ensures (vlparse lSize (vlbytes lSize vlb) == Correct vlb))
+  [SMTPat (vlparse lSize (vlbytes lSize vlb))]
+let vlparse_vlbytes lSize vlb =
+  let vl,b = split (vlbytes lSize vlb) lSize in
+  assert (Seq.equal vl (bytes_of_int lSize (length vlb)));
+  int_of_bytes_of_int lSize (length vlb);
+  match vlparse lSize (vlbytes lSize vlb) with
+  | Error z   -> ()
+  | Correct b -> lemma_vlbytes_inj lSize vlb b
+
+(** Serializing function for the certificate type *)
+val certTypeBytes: certType -> Tot (lbytes 1)
+let certTypeBytes ct =
+  match ct with
+  | RSA_sign     -> abyte 1z
+  | DSA_sign     -> abyte 2z
+  | RSA_fixed_dh -> abyte 3z
+  | DSA_fixed_dh -> abyte 4z
+
+(** Parsing function for the certificate type *)
+val parseCertType: pinverse_t certTypeBytes
+let parseCertType b =
+  match cbyte b with
+  | 1z -> Correct RSA_sign
+  | 2z -> Correct DSA_sign
+  | 3z -> Correct RSA_fixed_dh
+  | 4z -> Correct DSA_fixed_dh
+  | _ -> Error(AD_decode_error, perror __SOURCE_FILE__ __LINE__ "")
+
+
+(** Lemmas associated to serializing/parsing of certificate types *)
+val inverse_certType: x:_ -> Lemma
+  (requires (True))
+  (ensures lemma_inverse_g_f certTypeBytes parseCertType x)
+  [SMTPat (parseCertType (certTypeBytes x))]
+let inverse_certType x = ()
+
+val pinverse_certType: x:_ -> Lemma
+  (requires (True))
+  (ensures (lemma_pinverse_f_g Seq.equal certTypeBytes parseCertType x))
+  [SMTPat (certTypeBytes (Correct._0 (parseCertType x)))]
+let pinverse_certType x = ()
+
+
+#set-options "--max_fuel 1 --initial_fuel 1"
+
+(** Serializing function for lists of certificate types *)
+val certificateTypeListBytes: ctl:list certType -> Tot (lbytes (List.Tot.length ctl))
+let rec certificateTypeListBytes ctl =
+  match ctl with
+  | [] -> empty_bytes
+  | h::t ->
+    let ct = certTypeBytes h in
+    ct @| certificateTypeListBytes t
+
+(** Parsing function for lists of certificate types *)
+val parseCertificateTypeList: data:bytes -> Tot (list certType) (decreases (length data))
+let rec parseCertificateTypeList data =
+  if length data = 0 then []
+  else
+    let (thisByte,data) = Platform.Bytes.split data 1 in
+    match parseCertType thisByte with
+    | Error z -> // we skip this one
+      parseCertificateTypeList data
+    | Correct ct ->
+      let rem = parseCertificateTypeList data in
+      ct :: rem
+
+
+(** Serializing function for a list of Distinguished Names of certificates *)
+val distinguishedNameListBytes: names:list dn -> Tot (b:bytes{length b <= op_Multiply 258 (List.Tot.length names)})
+let rec distinguishedNameListBytes names =
+  match names with
+  | [] -> empty_bytes
+  | h::t ->
+    lemma_repr_bytes_values (length (utf8 h));
+    let name = vlbytes 2 (utf8 h) in
+    name @| distinguishedNameListBytes t
+
+(** Parsing function for a list of Distinguished Names of certificates *)
+val parseDistinguishedNameList: data:bytes -> res:list dn -> Tot (result (list dn)) (decreases (length data))
+let rec parseDistinguishedNameList data res =
+  if length data = 0 then
+    Correct res
+  else
+    if length data < 2 then
+      Error(AD_decode_error, perror __SOURCE_FILE__ __LINE__ "")
+    else
+      match vlsplit 2 data with
+      | Error z -> Error z
+      | Correct (nameBytes,data) ->
+        begin
+	match iutf8_opt nameBytes with
+        | None -> Error(AD_decode_error, perror __SOURCE_FILE__ __LINE__ "")
+        | Some name ->
+	  if length (utf8 name) < 256 then
+          let res = name :: res in
+          parseDistinguishedNameList data res
+	  else Error(AD_decode_error, perror __SOURCE_FILE__ __LINE__ "")
+        end
+
+(** Serializing function for (EC)DHE named groups *)
+val namedGroupBytes: namedGroup -> Tot (lbytes 2)
+let namedGroupBytes ng =
+  match ng with
+  | SEC ec ->
+    begin
+    match ec with
+    | ECC_P256		-> abyte2 (0x00z, 0x17z)
+    | ECC_P384		-> abyte2 (0x00z, 0x18z)
+    | ECC_P521		-> abyte2 (0x00z, 0x19z)
+    end
+  | EC_UNSUPPORTED b	-> abyte2 (0x00z, b)
+  | FFDHE dhe ->
+    begin
+    match dhe with
+    | FFDHE2048		-> abyte2 (0x01z, 0x00z)
+    | FFDHE3072		-> abyte2 (0x01z, 0x01z)
+    | FFDHE4096		-> abyte2 (0x01z, 0x02z)
+    | FFDHE6144		-> abyte2 (0x01z, 0x03z)
+    | FFDHE8192		-> abyte2 (0x01z, 0x04z)
+    end
+  | FFDHE_PRIVATE_USE b -> abyte2 (0x01z, b)
+  | ECDHE_PRIVATE_USE b -> abyte2 (0xFEz, b)
+
+(** Parsing function for (EC)DHE named groups *)
+val parseNamedGroup: pinverse_t namedGroupBytes
+let parseNamedGroup b =
+  match cbyte2 b with
+  | (0x00z, 0x17z) -> Correct (SEC ECC_P256)
+  | (0x00z, 0x18z) -> Correct (SEC ECC_P384)
+  | (0x00z, 0x19z) -> Correct (SEC ECC_P521)
+  | (0x00z, b)     -> Correct (EC_UNSUPPORTED b) // REMARK: only values 0x01z-0x16z and 0x1Az-0x1Ez are assigned
+  | (0x01z, 0x00z) -> Correct (FFDHE FFDHE2048)
+  | (0x01z, 0x01z) -> Correct (FFDHE FFDHE3072)
+  | (0x01z, 0x02z) -> Correct (FFDHE FFDHE4096)
+  | (0x01z, 0x03z) -> Correct (FFDHE FFDHE6144)
+  | (0x01z, 0x04z) -> Correct (FFDHE FFDHE8192)
+  | (0x01z, b)     ->
+    if b = 0xFCz || b = 0xFDz || b = 0xFEz || b = 0xFFz
+    then Correct (FFDHE_PRIVATE_USE b)
+    else Error (AD_decode_error, perror __SOURCE_FILE__ __LINE__ "Wrong ffdhe private use group")
+  | (0xFEz, b)     -> Correct (ECDHE_PRIVATE_USE b)
+  | _ -> Error (AD_decode_error, perror __SOURCE_FILE__ __LINE__ "Wrong named group")
+
+(** Lemmas for named groups parsing/serializing inversions *)
+val inverse_namedGroup: x:_ -> Lemma
+  (requires (True))
+  (ensures lemma_inverse_g_f namedGroupBytes parseNamedGroup x)
+  [SMTPat (parseNamedGroup (namedGroupBytes x))]
+let inverse_namedGroup x = ()
+
+val pinverse_namedGroup: x:_ -> Lemma
+  (requires (True))
+  (ensures (lemma_pinverse_f_g Seq.equal namedGroupBytes parseNamedGroup x))
+  [SMTPat (namedGroupBytes (Correct._0 (parseNamedGroup x)))]
+let pinverse_namedGroup x = ()
+
+
+private val namedGroupsBytes0: groups:list namedGroup
+  -> Tot (b:bytes { length b = op_Multiply 2 (List.Tot.length groups)})
+let rec namedGroupsBytes0 groups =
+  match groups with
+  | [] -> empty_bytes
+  | g::gs -> namedGroupBytes g @| namedGroupsBytes0 gs
+
+(** Serialization function for a list of named groups *)
+val namedGroupsBytes: groups:list namedGroup{List.Tot.length groups < 65536/2}
+  -> Tot (b:bytes { length b = 2 + op_Multiply 2 (List.Tot.length groups)})
+let namedGroupsBytes groups =
+  let gs = namedGroupsBytes0 groups in
+  lemma_repr_bytes_values (length gs);
+  vlbytes 2 gs
+
+private val parseNamedGroups0: b:bytes -> l:list namedGroup
+  -> Tot (result (groups:list namedGroup{List.Tot.length groups = List.Tot.length l + length b / 2}))
+  (decreases (length b))
+let rec parseNamedGroups0 b groups =
+  if length b > 0 then
+    if length b >= 2 then
+      let (ng, bytes) = split b 2 in
+      lemma_split b 2;
+      match parseNamedGroup ng with
+      |Correct ng ->
+        let groups' = ng :: groups in
+        parseNamedGroups0 bytes groups'
+      | Error z    -> Error z
+    else Error (AD_decode_error, perror __SOURCE_FILE__ __LINE__ "")
+  else
+   let grev = List.Tot.rev groups in
+   assume (List.Tot.length grev == List.Tot.length groups);
+   Correct grev
+
+(** Parsing function for a list of named groups *)
+val parseNamedGroups: b:bytes { 2 <= length b /\ length b < 65538 }
+  -> Tot (result (groups:list namedGroup{List.Tot.length groups = (length b - 2) / 2}))
+let parseNamedGroups b =
+  match vlparse 2 b with
+  | Correct b -> parseNamedGroups0 b []
+  | Error z   ->
+    Error(AD_decode_error, perror __SOURCE_FILE__ __LINE__ "Failed to parse named groups")
+
+
+(** Serializing function for the configuration identifier *)
+val configurationIdBytes: configurationId -> Tot (b:bytes{2 < length b /\ length b < 65538})
+let configurationIdBytes cid =
+  lemma_repr_bytes_values (length cid);
+  vlbytes 2 cid
+
+(** Parsing function for the configuration identifier *)
+val parseConfigurationId: pinverse_t configurationIdBytes
+let parseConfigurationId b =
+  match vlparse 2 b with
+  | Error z -> Error z
+  | Correct b -> Correct b
+
+(** Lemmas for configurationId serializing/parsing inversion *)
+val inverse_configurationId: x:_ -> Lemma
+  (requires (True))
+  (ensures lemma_inverse_g_f configurationIdBytes parseConfigurationId x)
+  [SMTPat (parseConfigurationId (configurationIdBytes x))]
+let inverse_configurationId x =
+  lemma_repr_bytes_values (length x)
+
+val pinverse_configurationId: x:_ -> Lemma
+  (requires (True))
+  (ensures (lemma_pinverse_f_g Seq.equal configurationIdBytes parseConfigurationId x))
+  [SMTPat (configurationIdBytes (Correct._0 (parseConfigurationId x)))]
+let pinverse_configurationId x = ()
+
+
+//
+// BB.TODO: Some of the following code should be moved outside TLSConstants !
+//          In particular, the integer definitions can be taken from F* ulib.
+
+type uint32 = b:lbytes 4
+
+val uint32Bytes: uint32 -> Tot (lbytes 4)
+let uint32Bytes u = u
+
+val parseUint32: pinverse_t uint32Bytes
+let parseUint32 b =
+  if length b = 4 then Correct(b)
+  else Error (AD_decode_error, perror __SOURCE_FILE__ __LINE__ "")
+
+val inverse_uint32: x:_ -> Lemma
+  (requires (True))
+  (ensures lemma_inverse_g_f uint32Bytes parseUint32 x)
+  [SMTPat (parseUint32 (uint32Bytes x))]
+let inverse_uint32 x = ()
+
+val pinverse_uint32: x:_ -> Lemma
+  (requires (True))
+  (ensures (lemma_pinverse_f_g Seq.equal uint32Bytes parseUint32 x))
+  [SMTPat (uint32Bytes (Correct._0 (parseUint32 x)))]
+let pinverse_uint32 x = ()
+
+
+
+(** Serializing function for Early Data values *)
+val earlyDataTypeBytes: earlyDataType -> Tot (lbytes 1)
+let earlyDataTypeBytes edt =
+  match edt with
+  | ClientAuthentication        -> abyte 1z
+  | EarlyData                   -> abyte 2z
+  | ClientAuthenticationAndData -> abyte 3z
+
+(** Parsing function for Early Data values *)
+val parseEarlyDataType: pinverse_t earlyDataTypeBytes
+let parseEarlyDataType b =
+  match cbyte b with
+  | 1z -> Correct ClientAuthentication
+  | 2z -> Correct EarlyData
+  | 3z -> Correct ClientAuthenticationAndData
+  | _  -> Error (AD_decode_error, perror __SOURCE_FILE__ __LINE__ "Failed to parse early data type")
+
+
+(** Lemmas for Early Data parsing/serializing inversions *)
+val inverse_earlyDataType: x:_ -> Lemma
+  (requires (True))
+  (ensures lemma_inverse_g_f earlyDataTypeBytes parseEarlyDataType x)
+  [SMTPat (parseEarlyDataType (earlyDataTypeBytes x))]
+let inverse_earlyDataType x = ()
+
+val pinverse_earlyDataType: x:_ -> Lemma
+  (requires (True))
+  (ensures (lemma_pinverse_f_g Seq.equal earlyDataTypeBytes parseEarlyDataType x))
+  [SMTPat (earlyDataTypeBytes (Correct._0 (parseEarlyDataType x)))]
+let pinverse_earlyDataType x = ()
+
+
+// TODO: Should we strengthen the result type to b:bytes{length b >= 4}?
+(** Serialization of the configuration extension values *)
+val configurationExtensionBytes: ce:configurationExtension -> Tot bytes
+let configurationExtensionBytes ce =
+  match ce with
+  | UnknownConfigurationExtension typ payload -> typ @| vlbytes 2 payload
+
+(** Parsing of the configuration extension values *)
+val parseConfigurationExtension: pinverse_t configurationExtensionBytes
+let parseConfigurationExtension b =
+  if length b >= 4 then
+    let (typ,payload) = split b 2 in
+    match vlparse 2 payload with
+    | Correct payload -> Correct (UnknownConfigurationExtension typ payload)
+    | Error z -> Error z
+  else Error (AD_decode_error, perror __SOURCE_FILE__ __LINE__ "Too few bytes to parse a configuration extension")
+
+
+(** Lemmas for Configuration Extension parsing/serializing inversions *)
+val inverse_configurationExtension: x:_ -> Lemma
+  (requires (True))
+  (ensures lemma_inverse_g_f configurationExtensionBytes parseConfigurationExtension x)
+  [SMTPat (parseConfigurationExtension (configurationExtensionBytes x))]
+let inverse_configurationExtension x =
+  match x with
+  | UnknownConfigurationExtension typ payload ->
+  let b = typ @| vlbytes 2 payload in
+  let b0,b1 = split b 2 in
+  let vl,b = split b1 2 in
+  vlparse_vlbytes 2 b;
+  assert (Seq.equal vl (bytes_of_int 2 (length b)));
+  assert (Seq.equal b0 typ);
+  assert (Seq.equal b payload)
+
+val pinverse_configurationExtension: x:_ -> Lemma
+  (requires (True))
+  (ensures (lemma_pinverse_f_g Seq.equal configurationExtensionBytes parseConfigurationExtension x))
+  [SMTPat (configurationExtensionBytes (Correct._0 (parseConfigurationExtension x)))]
+let pinverse_configurationExtension x = ()
+
+
+// TODO: Choice, truncate when maximum length is exceeded
+(** Serialization of the configuration extension list of values *)
+val configurationExtensionsBytes: list configurationExtension -> Tot bytes
+let configurationExtensionsBytes ce =
+  let rec configurationExtensionsBytes_aux (b:bytes{length b < 65536}) (ces:list configurationExtension): Tot (b:bytes{length b < 65536}) (decreases ces) =
+  match ces with
+  | [] -> b
+  | ce::ces ->
+    if length (b @| configurationExtensionBytes ce) < 65536 then
+      configurationExtensionsBytes_aux (b @| configurationExtensionBytes ce) ces
+    else b
+  in
+  let b = configurationExtensionsBytes_aux empty_bytes ce in
+  lemma_repr_bytes_values (length b);
+  vlbytes 2 b
+
+(** Parsing of the configuration extension list of values *)
+val parseConfigurationExtensions: pinverse_t configurationExtensionsBytes
+let parseConfigurationExtensions b =
+  let rec (aux: b:bytes -> list configurationExtension -> Tot (result (list configurationExtension)) (decreases (length b))) =
+    fun b exts ->
+    if length b > 0 then
+      if length b >= 4 then
+	let typ, len, data = split2 b 2 2 in
+	let len = int_of_bytes len in
+	if length b >= 4 + len then
+	  let ext, bytes = split b len in
+	  match parseConfigurationExtension ext with
+	  | Correct(ext') -> aux bytes (ext'::exts)
+	  | Error(z) -> Error(z)
+	else Error(AD_decode_error, perror __SOURCE_FILE__ __LINE__ "Failed to parse configuration extension length")
+      else Error(AD_decode_error, perror __SOURCE_FILE__ __LINE__ "Configuration extension length should be at least 4")
+    else Correct(exts) in
+  if length b >= 2 then
+  match vlparse 2 b with
+  | Correct (b) ->  aux b []
+  | Error(z) -> Error(AD_decode_error, perror __SOURCE_FILE__ __LINE__ "Failed to parse configuration extension")
+  else Error(AD_decode_error, perror __SOURCE_FILE__ __LINE__ "Failed to parse configuration extension")
+
+
+(** Serializing function for the Signature algorithm *)
+val sigHashAlgBytes: sigHashAlg -> Tot (lbytes 2)
+let sigHashAlgBytes sha =
+  let sign = sigAlgBytes (fst sha) in
+  let hash = hashAlgBytes (snd sha) in
+  hash @| sign
+
+val sigSchemeBytes: sigScheme -> Tot (lbytes 2)
+let sigSchemeBytes ss = 
+  match ss with
+  | SigHashAlg sha -> sigHashAlgBytes sha
+  | RSA_PSS_SHA256 -> abyte2(0x08z, 0x04z)
+  | RSA_PSS_SHA384 -> abyte2(0x08z, 0x05z)
+  | RSA_PSS_SHA512 -> abyte2(0x08z, 0x06z)
+  | ED25519 -> abyte2(0x08z, 0x07z)
+  | ED448 -> abyte2(0x08z, 0x08z)
+
+(** Parsing function for the Signature algorithm *)
+val parseSigHashAlg: pinverse_t sigHashAlgBytes
+let parseSigHashAlg b =
+  let hash,sign = split b 1 in
+  match parseSigAlg sign with
+  | Correct sign ->
+    begin
+    match parseHashAlg hash with
+    | Correct hash -> Correct(sign, hash)
+    | Error z -> Error z
+    end
+  | Error z -> Error z
+
+val parseSigScheme: pinverse_t sigSchemeBytes
+let parseSigScheme b = 
+  match cbyte2 b with
+  | (0x08z, 0x04z) -> Correct(RSA_PSS_SHA256)
+  | (0x08z, 0x05z) -> Correct(RSA_PSS_SHA384)
+  | (0x08z, 0x06z) -> Correct(RSA_PSS_SHA512)
+  | (0x08z, 0x07z) -> Correct(ED25519)
+  | (0x08z, 0x08z) -> Correct(ED448)
+  | _ -> (match parseSigHashAlg b with
+          | Error p -> Error p 
+	  | Correct(s,h) -> Correct(SigHashAlg(s,h)))
+    
+// TODO: Moving this inside sigHashAlgsBytes gives a `Bound term variable not found` error
+// See https://github.com/FStarLang/FStar/issues/533
+
+(** Serializing function for a Signature algorithm list *)
+val sigHashAlgsBytes: algs:list sigHashAlg{List.Tot.length algs < 65536/2}
+  -> Tot (b:bytes{2 <= length b /\ length b < 65538})
+let sigHashAlgsBytes algs =
+  let rec sigHashAlgsBytes_aux: b:bytes
+    -> algs:list sigHashAlg{b2t (length b + op_Multiply 2 (List.Tot.length algs) < 65536)}
+    -> Tot (r:bytes{length r < 65536}) (decreases algs) = fun b algs ->
+    match algs with
+    | [] -> b
+    | alg::algs' ->
+      let shb = sigHashAlgBytes alg in
+      sigHashAlgsBytes_aux (shb @| b) algs'
+  in
+  let b = sigHashAlgsBytes_aux empty_bytes algs in
+  lemma_repr_bytes_values (length b);
+  vlbytes 2 b
+
+(** Parsing function for a Signature algorithm list *)
+val parseSigHashAlgs: pinverse_t sigHashAlgsBytes
+let parseSigHashAlgs b =
+  let rec aux: b:bytes -> algs:list sigHashAlg{length b + op_Multiply 2 (List.Tot.length algs) < 65536} -> Tot (result (l:list sigHashAlg{List.Tot.length l < 65536/2})) (decreases (length b)) = fun b algs ->
+    if length b > 0 then
+      if length b >= 2 then
+      let alg,bytes = split b 2 in
+      match parseSigHashAlg alg with
+      | Correct sha -> aux bytes (sha::algs)
+      | Error z     -> Error z
+      else Error (AD_decode_error, perror __SOURCE_FILE__ __LINE__ "Too few bytes to parse sig hash algs")
+    else Correct algs in
+  match vlparse 2 b with
+  | Correct b -> aux b []
+  | Error z   -> Error(AD_decode_error, perror __SOURCE_FILE__ __LINE__ "Failed to parse sig hash algs")
+
+
+val sigSchemesBytes: algs:list sigScheme{List.Tot.length algs < 65536/2}
+  -> Tot (b:bytes{2 <= length b /\ length b < 65538})
+let sigSchemesBytes algs =
+  let rec sigSchemesBytes_aux: b:bytes
+    -> algs:list sigScheme{b2t (length b + op_Multiply 2 (List.Tot.length algs) < 65536)}
+    -> Tot (r:bytes{length r < 65536}) (decreases algs) = fun b algs ->
+    match algs with
+    | [] -> b
+    | alg::algs' ->
+      let shb = sigSchemeBytes alg in
+      sigSchemesBytes_aux (shb @| b) algs'
+  in
+  let b = sigSchemesBytes_aux empty_bytes algs in
+  lemma_repr_bytes_values (length b);
+  vlbytes 2 b
+
+val parseSigSchemes: pinverse_t sigSchemesBytes
+let parseSigSchemes b =
+  let rec aux: b:bytes -> algs:list sigScheme{length b + op_Multiply 2 (List.Tot.length algs) < 65536} -> Tot (result (l:list sigScheme{List.Tot.length l < 65536/2})) (decreases (length b)) = fun b algs ->
+    if length b > 0 then
+      if length b >= 2 then
+      let alg,bytes = split b 2 in
+      match parseSigScheme alg with
+      | Correct sha -> aux bytes (sha::algs)
+      | Error z     -> Error z
+      else Error (AD_decode_error, perror __SOURCE_FILE__ __LINE__ "Too few bytes to parse sig hash algs")
+    else Correct algs in
+  match vlparse 2 b with
+  | Correct b -> aux b []
+  | Error z   -> Error(AD_decode_error, perror __SOURCE_FILE__ __LINE__ "Failed to parse sig hash algs")
+
+
+(** Serializing function for a KeyShareEntry *)
+val keyShareEntryBytes: keyShareEntry -> Tot (b:bytes{4 <= length b})
+let keyShareEntryBytes (ng, b) =
+  let ng_bytes = namedGroupBytes ng in
+  ng_bytes @| vlbytes 2 b
+
+(** Parsing function for a KeyShareEntry *)
+val parseKeyShareEntry: pinverse_t keyShareEntryBytes
+let parseKeyShareEntry b =
+  let ng,key_exchange = split b 2 in
+  match parseNamedGroup ng with
+  | Correct ng ->
+    begin
+    match vlparse 2 key_exchange with
+    | Correct ke -> Correct (ng, ke)
+    | Error z    -> Error(AD_decode_error, perror __SOURCE_FILE__ __LINE__ "Failed to parse key share entry")
+    end
+  | Error z -> Error z
+
+
+(** Lemmas for KeyShare entries parsing/serializing inversions *)
+val inverse_keyShareEntry: x:_ -> Lemma
+  (requires (True))
+  (ensures lemma_inverse_g_f keyShareEntryBytes parseKeyShareEntry x)
+  [SMTPat (parseKeyShareEntry (keyShareEntryBytes x))]
+let inverse_keyShareEntry (ng, x) =
+  let b = namedGroupBytes ng @| vlbytes 2 x in
+  let b0,b1 = split b 2 in
+  let vl,b = split b1 2 in
+  vlparse_vlbytes 2 b;
+  assert (Seq.equal vl (bytes_of_int 2 (length b)));
+  assert (Seq.equal b0 (namedGroupBytes ng));
+  assert (Seq.equal b x)
+
+val pinverse_keyShareEntry: x:_ -> Lemma
+  (requires (True))
+  (ensures lemma_pinverse_f_g Seq.equal keyShareEntryBytes parseKeyShareEntry x)
+  [SMTPat (keyShareEntryBytes (Correct._0 (parseKeyShareEntry x)))]
+let pinverse_keyShareEntry x = ()
+
+
+// Choice: truncate when maximum length is exceeded
+(** Serializing function for a list of KeyShareEntry *)
+val keyShareEntriesBytes: list keyShareEntry -> Tot (b:bytes{2 <= length b /\ length b < 65538})
+let keyShareEntriesBytes kes =
+  let rec keyShareEntriesBytes_aux (b:bytes{length b < 65536}) (kes:list keyShareEntry): Tot (b:bytes{length b < 65536}) (decreases kes) =
+  match kes with
+  | [] -> b
+  | ke::kes ->
+    let b' = b @| keyShareEntryBytes ke in
+    if length b' < 65536 then
+      keyShareEntriesBytes_aux b' kes
+    else b
+  in
+  let b = keyShareEntriesBytes_aux empty_bytes kes in
+  lemma_repr_bytes_values (length b);
+  vlbytes 2 b
+
+(** Parsing function for a list KeyShareEntry *)
+val parseKeyShareEntries: pinverse_t keyShareEntriesBytes
+let parseKeyShareEntries b =
+  let rec (aux: b:bytes -> list keyShareEntry -> Tot (result (list keyShareEntry)) (decreases (length b))) = fun b entries ->
+    if length b > 0 then
+      if length b >= 4 then
+	let ng, data = split b 2 in
+	match vlsplit 2 data with
+	| Correct(kex, bytes) ->
+	  begin
+	  match parseKeyShareEntry (ng @| vlbytes 2 kex) with
+	  | Correct entry -> aux bytes (entries @ [entry])
+	  | Error z -> Error z
+	  end
+	| Error z -> Error(AD_decode_error, perror __SOURCE_FILE__ __LINE__ "Failed to parse key share entry")
+      else Error (AD_decode_error, perror __SOURCE_FILE__ __LINE__ "Too few bytes to parse key share entries")
+    else Correct entries in
+  match vlparse 2 b with
+  | Correct b -> aux b []
+  | Error z   -> Error(AD_decode_error, perror __SOURCE_FILE__ __LINE__ "Failed to parse key share entries")
+
+(** Serializing function for a ClientKeyShare *)
+val clientKeyShareBytes: clientKeyShare -> Tot (b:bytes{ 2 <= length b /\ length b < 65538 })
+let clientKeyShareBytes cks = keyShareEntriesBytes cks
+
+(** Parsing function for a ClientKeyShare *)
+val parseClientKeyShare: b:bytes{ 2 <= length b /\ length b < 65538 }
+  -> Tot (result clientKeyShare)
+let parseClientKeyShare b =
+  match parseKeyShareEntries b with
+  | Correct kes ->
+    if List.Tot.length kes < 65536/4
+    then Correct kes
+    else Error(AD_decode_error, perror __SOURCE_FILE__ __LINE__ "Failed to parse client key share entries")
+  | Error z -> Error z
+
+(** Serializing function for a ServerKeyShare *)
+val serverKeyShareBytes: serverKeyShare -> Tot (b:bytes{ 4 <= length b })
+let serverKeyShareBytes sks = keyShareEntryBytes sks
+
+(** Parsing function for a ServerKeyShare *)
+val parseServerKeyShare: pinverse_t serverKeyShareBytes
+let parseServerKeyShare b = parseKeyShareEntry b
+
+(** Serializing function for a KeyShare *)
+val keyShareBytes: keyShare -> Tot bytes
+let keyShareBytes = function
+  | ClientKeyShare cks -> clientKeyShareBytes cks
+  | ServerKeyShare sks -> serverKeyShareBytes sks
+
+(** Parsing function for a KeyShare *)
+val parseKeyShare: bool -> bytes -> Tot (result keyShare)
+let parseKeyShare is_client b =
+  if is_client then
+    begin
+    if 2 <= length b && length b < 65538 then
+      begin
+      match parseClientKeyShare b with
+      | Correct kse -> Correct (ClientKeyShare kse)
+      | Error z -> Error z
+      end
+    else Error(AD_decode_error, perror __SOURCE_FILE__ __LINE__ "Failed to parse key share")
+    end
+  else
+    if 4 <= length b then
+      begin
+      match parseServerKeyShare b with
+      | Correct ks -> Correct (ServerKeyShare ks)
+      | Error z -> Error z
+      end
+    else Error(AD_decode_error, perror __SOURCE_FILE__ __LINE__ "Failed to parse key share")
+
+(** Serializing function for a PSK Identity *)
+val pskIdentityBytes: pskIdentity -> Tot (b:bytes{length b >= 2})
+let pskIdentityBytes pski =
+  vlbytes 2 pski
+
+(** Parsing function for a PSK Identity *)
+val parsePskIdentity: pinverse_t pskIdentityBytes
+let parsePskIdentity b =
+  match vlparse 2 b with
+  | Correct vlb -> Correct vlb
+  | Error z -> Error(AD_decode_error, perror __SOURCE_FILE__ __LINE__ "Failed to parse psk_identity")
+
+
+// TODO: Choice, truncate when maximum length is exceeded
+
+(** Serializing function for a list of PSK Identity *)
+val pskIdentitiesBytes: list pskIdentity -> Tot (b:bytes{2 <= length b /\ length b < 65538})
+let pskIdentitiesBytes ids =
+  let rec pskIdentitiesBytes_aux (b:bytes{length b < 65536}) (ids:list pskIdentity): Tot (b:bytes{length b < 65536}) (decreases ids) =
+  match ids with
+  | [] -> b
+  | id::ids ->
+    let b' = b @| pskIdentityBytes id in
+    if length b' < 65536 then
+      pskIdentitiesBytes_aux b' ids
+    else b
+  in
+  let b = pskIdentitiesBytes_aux empty_bytes ids in
+  lemma_repr_bytes_values (length b);
+  vlbytes 2 b
+
+(** Parsing function for a list of PSK Identity *)
+val parsePskIdentities: pinverse_t pskIdentitiesBytes
+let parsePskIdentities b =
+  let rec (aux: b:bytes -> list pskIdentity -> Tot (result (list pskIdentity)) (decreases (length b))) = fun b ids ->
+    if length b > 0 then
+      if length b >= 2 then
+	let len, data = split b 2 in
+	let len = int_of_bytes len in
+	if length b >= len then
+	  let pski,bytes = split b len in
+	  if length pski >= 2 then
+   	    match parsePskIdentity pski with
+   	    | Correct id -> aux bytes (id::ids)
+   	    | Error z -> Error z
+	  else Error(AD_decode_error, perror __SOURCE_FILE__ __LINE__ "Failed to parse psk identity length")
+        else Error(AD_decode_error, perror __SOURCE_FILE__ __LINE__ "Failed to parse psk identity length")
+      else Error(AD_decode_error, perror __SOURCE_FILE__ __LINE__ "Expected psk identity to be at least 2 bytes long")
+    else Correct ids in
+  match vlparse 2 b with
+  | Correct b -> aux b []
+  | Error z   -> Error(AD_decode_error, perror __SOURCE_FILE__ __LINE__ "Failed to parse psk identities")
+
+
+(** Serializing function for ClientPreSharedKey *)
+val clientPreSharedKeyBytes: clientPreSharedKey -> Tot (b:bytes{ 2 <= length b /\ length b < 65538 })
+let clientPreSharedKeyBytes cpsk = pskIdentitiesBytes cpsk
+
+(** Parsing function for ClientPreSharedKey *)
+val parseClientPreSharedKey: b:bytes{ 2 <= length b /\ length b < 65538 }
+  -> Tot (result clientPreSharedKey)
+let parseClientPreSharedKey b =
+  match parsePskIdentities b with
+  | Correct ids ->
+    let l = List.Tot.length ids in
+    if 1 <= l && l < 65536/2
+    then Correct ids
+    else Error(AD_decode_error, perror __SOURCE_FILE__ __LINE__ "Failed to parse client psk identities")
+  | Error z -> Error z
+
+(** Serializing function for ServerPreSharedKey *)
+val serverPreSharedKeyBytes: serverPreSharedKey -> Tot (b:bytes{ 2 <= length b })
+let serverPreSharedKeyBytes cpsk = pskIdentityBytes cpsk
+
+(** Parsing function for ServerPreSharedKey *)
+val parseServerPreSharedKey: pinverse_t serverPreSharedKeyBytes
+let parseServerPreSharedKey b = parsePskIdentity b
+
+(** Serializing function for PreSharedKey *)
+val preSharedKeyBytes: preSharedKey -> Tot (b:bytes{length b >= 2})
+let preSharedKeyBytes = function
+  | ClientPreSharedKey cpsk -> clientPreSharedKeyBytes cpsk
+  | ServerPreSharedKey spsk -> serverPreSharedKeyBytes spsk
+
+(** Parsing function for PreSharedKey *)
+val parsePreSharedKey: pinverse_t preSharedKeyBytes
+let parsePreSharedKey b =
+  match vlparse 2 b with
+  | Correct b' ->
+    begin
+      match vlparse 2 b with
+      | Correct b'' -> // Client case
+	begin
+	if length b >= 2 && length b < 65538 then
+	  begin
+	  match parseClientPreSharedKey b with
+	  | Correct psks -> Correct (ClientPreSharedKey psks)
+	  | Error z -> Error z
+	  end
+	else Error(AD_decode_error, perror __SOURCE_FILE__ __LINE__ "Failed to parse  psk")
+	end
+      | Error _ -> // Server case
+	begin
+	match parseServerPreSharedKey b with
+	| Correct psk -> Correct (ServerPreSharedKey psk)
+	| Error z -> Error z
+	end
+    end
+  | Error z -> Error(AD_decode_error, perror __SOURCE_FILE__ __LINE__ "Failed to parse pre shared key")
+
+
+(* From DHGroup *)
+val serialize_dh: DHGroup.params -> DHGroup.share -> Tot bytes
+let serialize_dh dhp dh_Y =
+  lemma_repr_bytes_values (length (dhp.dh_p));
+  lemma_repr_bytes_values (length (dhp.dh_g));
+  lemma_repr_bytes_values (length dh_Y);
+  let pb  = vlbytes 2 dhp.dh_p in 
+  let gb  = vlbytes 2 dhp.dh_g in
+  let pkb = vlbytes 2 dh_Y in
+  pb @| gb @| pkb
+
+val serialize_dh_public: s:DHGroup.share -> len:nat{len < 65536 /\ length s <= len}
+  -> Tot (lbytes len)
+let serialize_dh_public dh_Y len =
+  let padded_dh_Y = createBytes (len - length dh_Y) 0z @| dh_Y in
+  lemma_repr_bytes_values len;
+  padded_dh_Y
+
+val parse_dh_public: p:bytes{2 <= length p} -> Tot (result DHGroup.share)
+let parse_dh_public p =
+  match vlparse 2 p with
+  | Correct n -> lemma_repr_bytes_values (length n); Correct n
+  | Error z -> Error z
+
+val parse_dh_partial: bytes -> Tot (result (DHGroup.key * bytes))
+let parse_dh_partial payload = 
+  if length payload >= 2 then
+    match vlsplit 2 payload with
+    | Error(z) -> Error(z)
+    | Correct(p, payload) ->
+      if length payload >= 2 then
+        match vlsplit 2 payload with
+        | Error(z) -> Error(z)
+        | Correct(g, payload) ->
+          if length payload >= 2 then
+            match vlsplit 2 payload with
+            | Error(z) -> Error(z)
+            | Correct(gy, rem) ->
+              if length gy <= length p then
+                let dhp = {dh_p = p; dh_g = g; dh_q = None; safe_prime = false} in
+                let dhk = {dh_params = dhp; dh_public = gy; dh_private = None} in
+                lemma_repr_bytes_values (length p);
+                lemma_repr_bytes_values (length g);
+                Correct (dhk,rem)
+              else Error(AD_decode_error, perror __SOURCE_FILE__ __LINE__ "")
+          else Error(AD_decode_error, perror __SOURCE_FILE__ __LINE__ "")
+      else Error(AD_decode_error, perror __SOURCE_FILE__ __LINE__ "")
+  else Error(AD_decode_error, perror __SOURCE_FILE__ __LINE__ "")
+
+
+(* From ECGroup *)
+val parse_curve: bytes -> Tot (option ECGroup.params)
+let parse_curve b =
+  if length b = 3 then
+    let (ty, id) = split b 1 in
+    if cbyte ty = 3z then
+      match cbyte2 id with
+      | (0z, 23z) -> Some (ECGroup.params_of_group ECC_P256)
+      | (0z, 24z) -> Some (ECGroup.params_of_group ECC_P384)
+      | (0z, 25z) -> Some (ECGroup.params_of_group ECC_P521)
+      | _ -> None
+    else None
+  else None
+
+val curve_id: ECGroup.params -> Tot (lbytes 2)
+let curve_id p =
+  abyte2 (match p.curve with
+  | ECC_P256 -> (0z, 23z)
+  | ECC_P384 -> (0z, 24z)
+  | ECC_P521 -> (0z, 25z))
+
+val parse_ec_point: ECGroup.params -> bytes -> Tot (option ECGroup.share)
+let parse_ec_point p b =
+  let clen = ec_bytelen p.curve in 
+  if length b = (op_Multiply 2 clen) + 1 then
+    let (et, ecxy) = split b 1 in
+    match cbyte et with
+    | 4z ->
+      let (x,y) = split ecxy clen in
+      let e = {ecx = x; ecy = y;} in
+      if CoreCrypto.ec_is_on_curve p e then Some e else None
+    |_ -> None
+  else None
+
+val parse_ec_partial: bytes -> Tot (TLSError.result ( ECGroup.key * bytes ))
+let parse_ec_partial payload = 
+    if length payload >= 7 then
+      let (curve, point) = split payload 3 in
+      match parse_curve curve with
+      | None -> Error(AD_decode_error, perror __SOURCE_FILE__ __LINE__ "Unsupported curve")
+      | Some(ecp) ->
+        match vlsplit 1 point with
+        | Error(z) -> Error(z)
+        | Correct(rawpoint, rem) ->
+           match parse_ec_point ecp rawpoint with
+           | None -> Error(AD_decode_error, perror __SOURCE_FILE__ __LINE__ ("Invalid EC point received:"^(Platform.Bytes.print_bytes rawpoint)))
+           | Some p -> Correct ({ec_params = ecp; ec_point = p; ec_priv = None},rem)
+    else Error(AD_decode_error, perror __SOURCE_FILE__ __LINE__ "")
+
+(* Assumes uncompressed point format for now (04||ecx||ecy) *) 
+val serialize_ec_point: p:ECGroup.params 
+  -> e:ECGroup.share{length e.ecx = ec_bytelen p.curve /\ length e.ecy = ec_bytelen p.curve}
+  -> Tot (b:bytes{length b = FStar.Mul(2 * ec_bytelen p.curve) + 1})
+let serialize_ec_point p e =
+  let pc = abyte 4z in
+  let x = pc @| e.ecx @| e.ecy in
+  x
+
+val serialize_ec: p:ECGroup.params
+  -> e:ECGroup.share{length e.ecx = ec_bytelen p.curve /\ length e.ecy = ec_bytelen p.curve}
+  -> Tot (b:bytes{length b = op_Multiply 2 (ec_bytelen p.curve) + 5})
+let serialize_ec ecp ecdh_Y =
+  let ty = abyte 3z in
+  let id = curve_id ecp in
+  let e = serialize_ec_point ecp ecdh_Y in
+  lemma_repr_bytes_values (length e);
+  let ve = vlbytes 1 e in
+  ty @| id @| ve
+
+
+(* KB: older more general code below 
+let getParams (c : ec_curve) : ec_params = 
+    let rawcurve : ec_prime = match c with
+    | ECC_P256 ->
+        {
+            ecp_prime = "115792089210356248762697446949407573530086143415290314195533631308867097853951";
+            ecp_order = "115792089210356248762697446949407573529996955224135760342422259061068512044369";
+            ecp_a = "115792089210356248762697446949407573530086143415290314195533631308867097853948"; // p-3
+            ecp_b = "5ac635d8aa3a93e7b3ebbd55769886bc651d06b0cc53b0f63bce3c3e27d2604b";
+            ecp_gx = "6b17d1f2e12c4247f8bce6e563a440f277037d812deb33a0f4a13945d898c296";
+            ecp_gy = "4fe342e2fe1a7f9b8ee7eb4a7c0f9e162bce33576b315ececbb6406837bf51f5";
+            ecp_bytelen = 32;
+            ecp_id = abyte2 (0z, 23z);
+        }
+    | ECC_P384 ->
+        {
+            ecp_prime = "39402006196394479212279040100143613805079739270465446667948293404245721771496870329047266088258938001861606973112319";
+            ecp_order = "39402006196394479212279040100143613805079739270465446667946905279627659399113263569398956308152294913554433653942643";
+            ecp_a = "39402006196394479212279040100143613805079739270465446667948293404245721771496870329047266088258938001861606973112316"; // p-3
+            ecp_b = "b3312fa7e23ee7e4988e056be3f82d19181d9c6efe8141120314088f5013875ac656398d8a2ed19d2a85c8edd3ec2aef";
+            ecp_gx = "aa87ca22be8b05378eb1c71ef320ad746e1d3b628ba79b9859f741e082542a385502f25dbf55296c3a545e3872760ab7";
+            ecp_gy = "3617de4a96262c6f5d9e98bf9292dc29f8f41dbd289a147ce9da3113b5f0b8c00a60b1ce1d7e819d7a431d7c90ea0e5f";
+            ecp_bytelen = 48;
+            ecp_id = abyte2 (0z, 24z);
+        }
+    | ECC_P521 ->
+        {
+            ecp_prime = "6864797660130609714981900799081393217269435300143305409394463459185543183397656052122559640661454554977296311391480858037121987999716643812574028291115057151";
+            ecp_order = "6864797660130609714981900799081393217269435300143305409394463459185543183397655394245057746333217197532963996371363321113864768612440380340372808892707005449";
+            ecp_a = "6864797660130609714981900799081393217269435300143305409394463459185543183397656052122559640661454554977296311391480858037121987999716643812574028291115057148"; // p-3
+            ecp_b = "051953eb9618e1c9a1f929a21a0b68540eea2da725b99b315f3b8b489918ef109e156193951ec7e937b1652c0bd3bb1bf073573df883d2c34f1ef451fd46b503f00";
+            ecp_gx = "0c6858e06b70404e9cd9e3ecb662395b4429c648139053fb521f828af606b4d3dbaa14b5e77efe75928fe1dc127a2ffa8de3348b3c1856a429bf97e7e31c2e5bd66";
+            ecp_gy = "11839296a789a3bc0045c8a5fb42c7d1bd998f54449579b446817afbd17273e662c97ee72995ef42640c550b9013fad0761353c7086a272c24088be94769fd16650";
+            ecp_bytelen = 66;
+            ecp_id = abyte2 (0z, 25z);
+        }
+    in { curve = EC_PRIME rawcurve; point_compression = false; }
+*)
+
+(* From CommonDH *)
+// Serialize in KeyExchange message format
+val serialize: CommonDH.key -> Tot bytes
+let serialize k = 
+  match k with
+  | CommonDH.FFKey k -> serialize_dh k.dh_params k.dh_public
+  | CommonDH.ECKey k -> serialize_ec k.ec_params k.ec_point
+
+val parse_partial: bytes -> bool -> Tot (TLSError.result (CommonDH.key * bytes)) 
+let parse_partial p ec = 
+  if ec then
+    begin
+    match parse_ec_partial p with
+    | Correct(eck,rem) -> Correct (CommonDH.ECKey eck, rem)
+    | Error z -> Error z
+    end
+  else
+    begin
+    match parse_dh_partial p with
+    | Correct(dhk,rem) -> Correct (CommonDH.FFKey dhk, rem)
+    | Error z -> Error z
+    end
+
+        
+  
+// Serialize for keyShare extension
+val serialize_raw: CommonDH.key -> Tot bytes
+let serialize_raw = function
+  | CommonDH.ECKey k -> serialize_ec_point k.ec_params k.ec_point
+  | CommonDH.FFKey k -> serialize_dh_public k.dh_public (length k.dh_params.dh_p)
+
+val parse: CommonDH.params -> bytes -> Tot (option CommonDH.key)
+let parse p x =
+  match p with
+  | CommonDH.ECP p -> 
+    begin
+    match parse_ec_point p x with 
+    | Some eck -> Some (CommonDH.ECKey ({ec_params=p; ec_point=eck; ec_priv=None;})) 
+    | None -> None
+    end
+  | CommonDH.FFP p ->
+    if length x = length p.dh_p then
+      Some (CommonDH.FFKey ({dh_params = p; dh_public = x; dh_private = None;}))
+    else None
+
+(* From Cert *)
+(* ------------------------------------------------------------------------ *)
+
+abstract val certificateListBytes: chain -> Tot bytes
+let rec certificateListBytes l =
+  match l with
+  | [] -> empty_bytes
+  | c::r -> 
+    lemma_repr_bytes_values (length c);
+    (vlbytes 3 c) @| (certificateListBytes r)
+
+val certificateListBytes_is_injective: c1:chain -> c2:chain ->
+  Lemma (Seq.equal (certificateListBytes c1) (certificateListBytes c2) ==> c1 == c2)
+let rec certificateListBytes_is_injective c1 c2 =
+  match c1, c2 with
+  | [], [] -> ()
+  | hd::tl, hd'::tl' ->
+    if certificateListBytes c1 = certificateListBytes c2 then
+      begin
+      lemma_repr_bytes_values (length hd); lemma_repr_bytes_values (length hd');
+      cut(Seq.equal ((vlbytes 3 hd) @| (certificateListBytes tl)) ((vlbytes 3 hd') @| (certificateListBytes tl')));
+      lemma_repr_bytes_values (length hd);
+      lemma_repr_bytes_values (length hd');
+      cut(Seq.equal (Seq.slice (vlbytes 3 hd) 0 3) (Seq.slice (certificateListBytes c1) 0 3));
+      cut(Seq.equal (Seq.slice (vlbytes 3 hd') 0 3) (Seq.slice (certificateListBytes c1) 0 3));
+      vlbytes_length_lemma 3 hd hd';
+      lemma_append_inj (vlbytes 3 hd) (certificateListBytes tl) (vlbytes 3 hd') (certificateListBytes tl');
+      lemma_vlbytes_inj 3 hd hd';
+      certificateListBytes_is_injective tl tl'
+      end
+  | [], hd::tl ->
+    begin
+    cut (length (certificateListBytes c1) = 0);
+    lemma_repr_bytes_values (length hd);
+    cut (Seq.equal (certificateListBytes c2) ((vlbytes 3 hd) @| (certificateListBytes tl)));
+    lemma_vlbytes_len 3 hd
+    end
+  | hd::tl, [] ->
+    begin
+    cut (length (certificateListBytes c2) = 0);
+    lemma_repr_bytes_values (length hd);
+    cut (Seq.equal (certificateListBytes c1) ((vlbytes 3 hd) @| (certificateListBytes tl)));
+    lemma_vlbytes_len 3 hd
+    end
+
+abstract val parseCertificateList: b:bytes -> Tot (result chain) (decreases (length b))
+let rec parseCertificateList b =
+  if length b >= 3 then
+    match vlsplit 3 b with
+    | Correct (c,r) ->
+      cut (repr_bytes (length c) <= 3);
+      let rl = parseCertificateList r in
+      begin
+      match rl with
+      | Correct x -> (lemma_repr_bytes_values (length c); Correct (c::x))
+      | e -> e
+      end
+    | _ -> Error(AD_bad_certificate_fatal, perror __SOURCE_FILE__ __LINE__ "Badly encoded certificate list")
+  else if length b = 0 then Correct []
+  else Error(AD_bad_certificate_fatal, perror __SOURCE_FILE__ __LINE__ "Badly encoded certificate list")
+
+val lemma_parseCertificateList_length: b:bytes -> 
+  Lemma (ensures (match parseCertificateList b with
+		  | Correct ces -> length (certificateListBytes ces) = length b
+		  | _ -> True))
+	(decreases (length b))
+let rec lemma_parseCertificateList_length b = 
+  match parseCertificateList b with
+  | Correct [] -> ()
+  | Correct (hd::tl) ->
+    begin
+    cut(length b >= 3);
+    match vlsplit 3 b with
+    | Correct (c, r) -> lemma_parseCertificateList_length r
+    | _ -> ()
+    end
+  | Error _ -> ()
+
